add caml types

theories/Interpreter.v
@@ -1,126 +1,124 @@
 Require Import ssreflect.
 
-Require Import ZArith Array.PArray List String Floats.
+Require Import ZArith Array.PArray List String Floats Lia.
 Require Ascii.
 Require Uint63.
 Import ListNotations.
 Open Scope string_scope.
 
-Require Import Malfunction.Malfunction Malfunction.Deserialize Malfunction.Serialize Ceres.Ceres Malfunction.Ceres.CeresSerialize Malfunction.Ceres.CeresFormat.
+Require Import Malfunction.Malfunction Malfunction.Deserialize Malfunction.SemanticsSpec Malfunction.Serialize Malfunction.Serialize Ceres.Ceres Malfunction.Ceres.CeresSerialize Malfunction.Ceres.CeresFormat.
+
 From MetaCoq Require Import bytestring.
 Open Scope bs.
 
-(* type value = *)
-(* | Block of int * value array *)
-(* | Vec of vector_type * value array *)
-(* | Func of (value -> value) *)
-(* | Int of inttype * Z.t *)
-(* | Float of float *)
-(* | Thunk of value Lazy.t *)
-#[bypass_check(positivity)]
-Inductive break : Prop :=
-| B : (break -> break) -> break.
+From Coq Require Import Uint63.
 
-Fixpoint prv (b : break) : False :=
-  match b with
-  | B f => prv (f (B f))
-  end.
+Class Heap := {
+  pointer : Type;
+  heapGen : forall (value : Type), Type;
+  fresh : forall {value : Type}, heapGen value -> pointer * heapGen value;
+  deref : forall {value : Type}, heapGen value -> pointer -> array value;
+  update : forall {value : Type}, heapGen value -> pointer -> array value -> heapGen value
+}.
 
-Goal False.
-Proof.
-  exact (prv (B (fun x => x))).
-Qed.
+Definition CanonicalHeap : Heap := 
+{| pointer := int ;
+   heapGen := fun value => (int * (int -> array value))%type;
+   fresh :=  fun _ '(max_ptr , h) => let ptr := Int63.add max_ptr (int_of_nat 1) in (ptr ,(ptr, h));
+   deref :=  fun _ '(_,h) ptr => h ptr;
+   update := fun _ '(max_ptr , h) ptr arr => (max_ptr , fun ptr' => if Int63.eqb ptr ptr' then arr else h ptr) |}. 
 
-#[bypass_check(positivity)]
-Inductive break_ : forall X : Prop, Prop :=
-| B_ (X : Prop) : (X -> break_ (break_ X)) -> break_ X.
+ Inductive rec_value `{Heap} := 
+   | RFunc of Ident.t * t
+   | RThunk of pointer
+   | Bad_recursive_value.
+ 
+ Inductive value `{Heap} :=
+ | Block of int * array value
+ | Vec of vector_type * pointer
+ | BString of vector_type * pointer
+ | Func of @Ident.Map.t value * Ident.t *  t
+ | RClos of @Ident.Map.t value * list Ident.t * list rec_value * nat
+ | Lazy of @Ident.Map.t value * t
+ | value_Int of inttype * Z
+ | Float of float
+ | Thunk of pointer
+ | fail of string
+ | not_evaluated
+ .
 
-Fixpoint prv_ {X : Prop} (x : X) (b : break_ X) : False.
-Proof.
-  destruct b.
-  eapply prv_.
-  2: eapply H; eauto. 
-  econstructor. eauto.
-Qed.
+Definition heap `{Heap} := heapGen value.
 
-Goal ~ (forall P, P \/ ~ P).
-Proof.
-  intros lem.
-  unshelve eapply prv_. exact True. eauto.
-  destruct (lem (break_ True)) as [H | H].
-  - exact H.
-  - econstructor. econstructor. eauto.
-    intros h. destruct H. eauto.
-Qed.
+Definition is_not_evaluated `{Heap} : value -> bool := 
+  fun v => match v with | not_evaluated => true | _ => false end. 
 
-#[bypass_check(positivity)]
-Inductive value :=
-| Block of int * array value      
-| Vec of vector_type * array value
-| Func of (value -> value)
-| value_Int of inttype * Z
-| Float of float
-| Thunk of value
-| fail of string
-.
-Scheme foo := Induction for value Sort Prop.
-Print foo.
-
-Definition add (x : string) (v : value) (locals : string -> value)  :=
+Definition add `{Heap} (x : string) (v : value) (locals : string -> value)  :=
   fun y =>
     if String.eqb y x then v else locals y.
-
-Definition option_def {A} (a : A) (x : option A) : A :=
-  match x with
-  | None => a
-  | Some a => a
-  end.
 
 Fixpoint Array_of_List' {A} count (l : list A) (a : array A) :=
   match l with
   | [] => a
-  | x :: l => Array_of_List' (S count) l (PArray.set a (Int63.of_Z (Z.of_nat count)) x)
+  | x :: l => Array_of_List' (S count) l (PArray.set a (int_of_nat count) x)
   end.
 
 Definition Array_of_list {A} (def : A) (l : list A) :=
-  Array_of_List' 0 l (PArray.make (Int63.of_Z (Z.of_nat (List.length l))) def).
+  Array_of_List' 0 l (PArray.make (int_of_nat (List.length l)) def).
 
 Definition Array_init {A} (size : int) f :=
-  let g := fun x => (f (Int63.of_Z (Z.of_nat x))) in
+  let g := fun x => (f (int_of_nat x)) in
   @Array_of_list A (g 0) (map g (seq 0 (Z.to_nat (Int63.to_Z size)))).
 
-Definition inttype_eqb (t1 t2 : inttype) :=
-  match t1, t2 with
-  | Int, Int
-  | Int32, Int32
-  | Int64, Int64
-  | Bigint, Bigint => true
-  | _, _ => false
+Definition as_ty `{Heap} ty := fun ty2 =>
+  match ty2 with
+  | value_Int (ty', n) => if inttype_eqb ty ty' then n else fail_Z "integer type missmatch"
+  | _ => fail_Z "expected integer"
   end.
 
-Definition vector_type_eqb (t1 t2 : vector_type) :=
-  match t1, t2 with
-  | Array, Array
-  | Bytevec, Bytevec => true
-  | _, _ => false
+Definition as_float `{Heap} x := match x with
+  | Float f => f
+  | _ => fail_float "expected float64"
+end.
+
+Definition RFunc_build `{Heap} recs := 
+    map (fun t =>
+      match t with 
+      Mlambda ([x], e) => RFunc (x , e)
+    | Mlambda (x :: xs , e) => RFunc (x , Mlambda (xs , e))
+    | _ => Bad_recursive_value
+    end) 
+    recs.
+
+Definition add_recs `{Heap} locals (self : list Ident.t) rfunc := 
+    mapi (fun n x => (x , RClos (locals, self, rfunc, n))) self.
+
+Definition add_self `{Heap} self rfunc locals := 
+    List.fold_left (fun l '(x,t) => Ident.Map.add x t l) (add_recs locals self rfunc) locals.
+
+Fixpoint map_acc {A B S: Type} (f : S -> A -> S * B) (s:S) (l : list A) : S * list B :=
+  match l with
+  | [] => (s , [])
+  | a :: t => let (s',b) := f s a in 
+              let (s'',bs) := map_acc f s' t in (s'', b :: bs)
   end.
 
-Definition fail_def {A} (a : A) (s : string) : A.
-  exact a.
-Qed.
+ Definition cond `{Heap} scr case : bool := 
+    (match case, scr with
+      | Tag n, Block (n', _) => Int63.eqb n n'
+      | Deftag, Block _ => true
+      | Intrange (min, max), value_Int (Int, n) => Z.leb (Int63.to_Z min) n && Z.leb n (Int63.to_Z max)
+      | _, _ => false end).
+  
+Definition find_match `{Heap} (interpret : heap -> @Ident.Map.t value -> @Ident.Map.t value -> t -> heap * value)
+:= fun h iglobals ilocals scr => fix find_match x := match x with
+| (cases, e) :: rest =>
+    if List.existsb (cond scr)  cases then
+      interpret h iglobals ilocals e
+    else
+      find_match rest
+| [] => (h, fail "no case matches") end.
 
-Definition fail_float := fail_def infinity.
-Definition fail_Z := fail_def Z.zero.
-
-Definition bitwidth := fun t =>
-  match t with
-  | Int => 63
-  | Int32 => 32
-  | Int64 => 64
-  | BigInt => fail_Z "no bitwidth for bigint"
-  end%Z.
-
-Definition truncate ty n :=
+Definition truncate `{Heap} ty n :=
   value_Int (ty, match ty with
                  | Bigint => n
                  | ty =>
@@ -132,6 +130,7 @@ Definition truncate ty n :=
                        Z.sub masked range
                  end).
 
+<<<<<<< HEAD
 Definition as_ty ty := fun ty2 =>
   match ty2 with
   | value_Int (ty', n) => if inttype_eqb ty ty' then n else fail_Z "integer type missmatch"
@@ -193,6 +192,8 @@ Definition int_of_nat n := Uint63.of_Z (Coq.ZArith.BinInt.Z.of_nat n).
 #[export] Instance Serialize_int : Serialize int := 
    fun i => to_sexp (Int63.to_Z i).
 
+=======
+>>>>>>> 30435f2 (add caml types)
 #[bypass_check(guard)]
 Fixpoint to_sexp_value (a : value) : sexp :=
   match a with
@@ -208,74 +209,76 @@ Fixpoint to_sexp_value (a : value) : sexp :=
 #[export] Instance Serialize_value : Serialize value := to_sexp_value.
 
 #[bypass_check(guard)]
-Fixpoint interpret
+Fixpoint interpret `{Heap} (h : heap)
+         (globals : @Ident.Map.t value)
          (locals : @Ident.Map.t value)
-         (x : t) {struct x} : value :=
+         (x : t) {struct x} : heap * value :=
   match x with
-  | Mvar v => Ident.Map.find v locals
+  | Mvar v => (h, Ident.Map.find v locals)
   | Mlambda (xs, e) =>
-    let (x, e) := match xs with
-     | [ ] => fail_def ("", Mvar "") "assert false"
-     | [x] => (x, e)
-     | x :: xs => (x, Mlambda (xs, e))
-    end in
-    Func (fun v => interpret (Ident.Map.add x v locals) e)
+    (h, match xs with
+    | [ ] => fail "assert false"
+    | x :: xs => 
+      let (x , e) := match xs with 
+        | [] => (x , e)
+        | _ :: _ => (x , Mlambda (xs, e)) end 
+      in Func (locals, x , e)
+    end)
   | Mapply (f_, vs) =>
      List.fold_left (fun f v => match f with
-     | Func f => f (interpret locals v)
-     | v_wrong => fail ("not a function: " ++ (to_string f_) ++ " evaluated to: " ++ (to_string v_wrong)) end) vs (interpret locals f_)
-  | Mlet (bindings, body) =>
+     | (h , Func (locals', x, e)) => 
+        let (h' , v') := interpret h globals locals v 
+        in interpret h' globals (Ident.Map.add x v' locals') e
+     | (h , (RClos (locals', self, mfix , n))) =>
+        let (h' , v') := interpret h globals locals v in
+        match nth n mfix Bad_recursive_value with
+        | RFunc (y , e) => 
+          interpret h' globals (Ident.Map.add y v' (add_self self mfix locals')) e
+        | _ => (h', fail "not a function") end
+     | (h , _) => (h , fail ("not a function: " ++ " evaluated to: ")) end) vs 
+      (interpret h globals locals f_)
+   | Mlet (bindings, body) =>
      let bind :=
-        fix bind (locals : @Ident.Map.t value) (bindings : list binding) : value :=
+        fix bind (h : heap) (locals : @Ident.Map.t value) (bindings : list binding) : heap * value :=
         match bindings with
-        | [] => interpret locals body
+        | [] => interpret h globals locals body
         | Unnamed e :: bindings => 
-           let _ := interpret locals e in bind locals bindings
+          let (h' , _) := interpret h globals locals e in bind h' locals bindings
         | Named (x, e) :: bindings =>
-           let locals := Ident.Map.add x (interpret locals e) (locals) in
-           bind locals bindings
+          let (h' ,v) := interpret h globals locals e in
+          bind h' (Ident.Map.add x v (locals)) bindings
         | Recursive recs :: bindings =>
-           let newlocals := newlocals interpret recs locals
-            in
-             bind newlocals bindings 
+          let self := map fst recs in
+          let rfunc := RFunc_build (map snd recs) in
+          bind h (add_self self rfunc locals) bindings 
         end
      in
-      bind locals bindings 
-  | Mnum (numconst_Int n) => value_Int (Int, Int63.to_Z n)
-  (* | Mnum (`Int32 n) -> Int (`Int32, Z.of_int32 n) *)
-  (* | Mnum (`Int64 n) -> Int (`Int64, Z.of_int64 n) *)
-  | Mnum (numconst_Bigint n) => value_Int (Bigint, n)
-  | Mnum (numconst_Float64 f) => Float f
+      bind h locals bindings 
+  | Mnum (numconst_Int n) => (h , value_Int (Int, Int63.to_Z n))
+  | Mnum (numconst_Bigint n) => (h , value_Int (Bigint, n))
+  | Mnum (numconst_Float64 f) => (h, Float f)
 
   | Mstring s =>
-     Vec (Bytevec,
-           Array_init (Int63.of_Z (Z.of_nat (String.length s))) (fun i => value_Int (Int, (Z.of_nat (Ascii.nat_of_ascii (option_def Ascii.Space (String.get (Z.to_nat (Int63.to_Z i)) (String.to_string s))))))))
+    let (ptr,h') := fresh h in
+    let str := Array_init (Int63.of_Z (Z.of_nat (String.length s))) 
+                      (fun i => value_Int (Int, (Z.of_nat (Ascii.nat_of_ascii (option_def Ascii.Space (String.get (Z.to_nat (Int63.to_Z i)) s)))))) in
+     (update h' ptr str , Vec (Bytevec, ptr))
+     
+  | Mglobal v => (h , Ident.Map.find v globals)
 
-  | Mglobal v => Ident.Map.find v locals
-
-  | Mswitch (scr, cases) =>
-      let scr := interpret locals scr in
-      let fix find_match x := match x with
-        | (cases, e) :: rest =>
-            if List.existsb (fun case => match case, scr with
-            | Tag n, Block (n', _) => Int63.eqb n n'
-            | Deftag, Block _ => true
-            | Intrange (min, max), value_Int (Int, n) => Z.leb (Int63.to_Z min) n && Z.leb n (Int63.to_Z max)
-            | _, _ => false end) cases then
-              interpret locals e
-            else
-              find_match rest
-        | [] => fail "no case matches" end in
-      find_match cases
+  | Mswitch (scr, cases) => 
+      let (h', scr') := interpret h globals locals scr in
+      find_match interpret h' globals locals scr' cases
 
   | Mnumop1 (op, embed_inttype ty, e) =>
-      let n := as_ty ty (interpret locals e) in
-      truncate ty (match op with Neg => Z.mul (-1) n | Not => Z.lnot n end)
+      let (h',v) := interpret h globals locals e in 
+      let n := as_ty ty v in
+      (h', truncate ty (match op with Malfunction.Neg => Z.mul (-1) n | Not => Z.lnot n end))
 
   | Mnumop2 (op, embed_inttype ty, e1, e2) =>
-      let e1 := interpret locals e1 in
-      let e2 := interpret locals e2 in
-      match op with
+      let (h1 , e1) := interpret h globals locals e1 in
+      let (h2 , e2) := interpret h1 globals locals e2 in
+      (h2, match op with
       | embed_binary_arith_op op =>
           let f := match op with
                    | Add => Z.add | Sub => Z.sub
@@ -309,24 +312,28 @@ Fixpoint interpret
             | Eq => comparison_eqb cmp Datatypes.Eq
                      end in
           value_Int (Int, if res then 1%Z else 0%Z)
-      end
-  | Mnumop1 (Neg, Float64, e) =>
-      Float (- as_float (interpret locals e))
+      end)
+  | Mnumop1 (Malfunction.Neg, Float64, e) =>
+    let (h' , v) := interpret h globals locals e in (h' , Float (- as_float v))
   | Mnumop1 (Not, Float64, _) 
   | Mnumop2 (embed_binary_bitwise_op _, Float64, _, _) =>
-      fail "invalid bitwise float operation"
+      (h , fail "invalid bitwise float operation")
   | Mnumop2 (embed_binary_arith_op op, Float64, e1, e2) =>
-      let e1 := as_float (interpret locals e1) in
-      let e2 := as_float (interpret locals e2) in
-      Float (match op with
+      let (h1,e1') := interpret h globals locals e1 in
+      let (h2,e2') := interpret h1 globals locals e2 in
+      let e1 := as_float e1' in
+      let e2 := as_float e2' in
+      (h2, Float (match op with
              | Add => e1 + e2
              | Sub => e1 - e2
              | Mul => e1 * e2
              | Div => e1 / e2
-             | Mod => fail_float "mod on floats not supported" end)
+             | Mod => fail_float "mod on floats not supported" end))
   | Mnumop2 (embed_binary_comparison op, Float64, e1, e2) =>
-      let e1 := as_float (interpret locals e1) in
-      let e2 := as_float (interpret locals e2) in
+      let (h1,e1') := interpret h globals locals e1 in
+      let (h2,e2') := interpret h1 globals locals e2 in
+      let e1 := as_float e1' in
+      let e2 := as_float e2' in
       let res := match op with
              | Lt => PrimFloat.ltb e1 e2
              | Gt => PrimFloat.ltb e2 e2
@@ -334,84 +341,599 @@ Fixpoint interpret
              | Gte => PrimFloat.leb e2 e1
              | Eq => PrimFloat.eqb e1 e2
                  end in
-      value_Int (Int, if res then 1%Z else 0%Z)
-
+      (h2, value_Int (Int, if res then 1%Z else 0%Z))
   | Mconvert (embed_inttype src, embed_inttype dst, e) =>
-      truncate dst (as_ty src (interpret locals e))
+      let (h',v) := interpret h globals locals e in
+      (h', truncate dst (as_ty src v))
   | Mconvert (embed_inttype src, Float64, e) =>
-      Float (PrimFloat.of_uint63 (Int63.of_Z (as_ty src (interpret locals e))))
+      let (h',v) := interpret h globals locals e in
+      (h',Float (PrimFloat.of_uint63 (Int63.of_Z (as_ty src v))))
   | Mconvert (Float64, Float64, e) =>
-      Float (as_float (interpret locals e))
+      let (h',v) := interpret h globals locals e in
+      (h',Float (as_float v))
   | Mvecnew (ty, len, def) =>
-      match ty, interpret locals len, interpret locals def with
+      let (h1,len') := interpret h globals locals len in
+      let (h2,def') := interpret h1 globals locals def in
+      let (ptr,h3) := fresh h2 in
+      match ty, len' , def' with
       | Array, value_Int (Int, len), v =>
-          Vec (Array, PArray.make (Int63.of_Z len) v)
+          (update h3 ptr (PArray.make (Int63.of_Z len) v), Vec (Array, ptr))
       | Bytevec, value_Int (Int, len), (value_Int (Int, k)) as v =>
           if Z.leb 0%Z k && Z.ltb k 256 then
-            Vec (Bytevec, PArray.make (Int63.of_Z len) v)
+            (update h3 ptr (PArray.make (Int63.of_Z len) v), Vec (Bytevec, ptr))
           else
-            fail "bad vector creation"
-      | _, _, _ => fail "bad vector creation"
+            (h3,fail "bad vector creation")
+      | _, _, _ => (h2,fail "bad vector creation")
       end
   | Mvecget (ty, vec, idx) =>
-      (match interpret locals vec, interpret locals idx with
-       | Vec (ty', vals), value_Int (Int,i) =>
+      let (h1,vec') := interpret h globals locals vec in
+      let (h2,idx') := interpret h1 globals locals idx in
+      (h2, match vec', idx' with
+       | Vec (ty', ptr), value_Int (Int,i) =>
            if vector_type_eqb ty ty' then
-             if Z.leb 0 i && Z.ltb i (Int63.to_Z (PArray.length vals)) then
-               PArray.get vals (Int63.of_Z i)
+             if Z.leb 0 i && Z.ltb i (Int63.to_Z (PArray.length (deref h ptr))) then
+               PArray.get (deref h ptr) (Int63.of_Z i)
              else
                fail "index out of bounds: %d"
            else
              fail "wrong vector type"
        | _, _ => fail "wrong vector type"
-       end
-      )
-  | Mvecset (ty, vec, idx, e) => fail "not implemented"
-      (* (match interpret locals vec, *)
-      (*        interpret locals idx, *)
-      (*        interpret locals e with *)
-      (*  | Vec (ty', vals), value_Int (Int, i), v => *)
-      (*      if vector_type_eqb ty ty' then *)
-      (*        let i := Int63.to_Z i in *)
-      (*        if Int63.leb (Int63.of_int 0) i && Int63.leb i (PArray.length vals) then *)
-      (*          match ty, v with *)
-      (*          | Array, _ => tt *)
-      (*          | Bytevec, Int (Int, i) *)
-  (*      else fail "wrong vector type" *)
-  | Mveclen (ty, vec) =>
-      match interpret locals vec with
-      | Vec (ty', vals) =>
-          if vector_type_eqb ty ty' then value_Int (Int, Int63.to_Z (PArray.length vals)) else fail "wrong vector type"
-      | _ => fail "wrong vector type"
+       end)      
+  | Mvecset (ty, vec, idx, e) => 
+      let (h1,vec') := interpret h globals locals vec in
+      let (h2,idx') := interpret h1 globals locals idx in
+      let (h3,v) := interpret h1 globals locals e in
+      match vec', idx', v with 
+        | Vec (ty', ptr), value_Int (Int, i), v => 
+          if vector_type_eqb ty ty' then 
+              let i := Int63.of_Z i in 
+              if Int63.leb (int_of_nat 0) i && Int63.leb i (PArray.length (deref h ptr)) then 
+                match ty, v with 
+                | Array, _ => (update h3 ptr (PArray.set (deref h ptr) i v), value_Int (Int, 0%Z))
+                | Bytevec, value_Int (Int, val) => 
+                  if (Z.leb 0 val) && (Z.ltb val 256)
+                  then 
+                    (update h3 ptr (PArray.set (deref h ptr) i v), value_Int (Int, 0%Z))
+                  else (h3, fail "not a byte")
+                | Bytevec, _ => (h3, fail "not a byte")
+                end 
+              else (h3, fail "index out of bounds: %d")
+          else (h3, fail "wrong vector type")
+        | _ , _ , _ => (h3, fail "wrong vector type")
       end
+  | Mveclen (ty, vec) =>
+      let (h',vec') := interpret h globals locals vec in
+      (h', match vec' with
+      | Vec (ty', ptr) =>
+          if vector_type_eqb ty ty' then value_Int (Int, Int63.to_Z (PArray.length (deref h ptr)))
+                                    else fail "wrong vector type"
+      | _ => fail "wrong vector type"
+      end)
   | Mblock (tag, vals) =>
-      Block (tag, Array_of_list (fail "") (List.map (interpret locals) vals))
+      let (h',vals') := map_acc (fun h e => interpret h globals locals e) h vals in
+      (h', if (int_of_nat (Datatypes.length vals) ≤? max_length)%uint63 
+           then Block (tag, Array_of_list (fail "") vals')
+           else fail "vals is a too big array")
   | Mfield (idx, b) =>
-      match interpret locals b with
+      let (h',b') := interpret h globals locals b in
+      (h', match b' with
       | Block (_, vals) => PArray.get vals idx
       | _ => fail "not a block"
-      end
-  | Mlazy e => Thunk (interpret locals e)
+      end)
+  | Mlazy e => 
+    let (ptr,h') := fresh h in
+    let init := PArray.make (Int63.of_Z 2) not_evaluated in
+    let arr := PArray.set init (Int63.of_Z 1) (Lazy (locals , e)) in
+    (update h' ptr arr, Thunk ptr)
   | Mforce e =>
-      match interpret locals e with
-      | Thunk v => v
-      | _ => fail "not a lazy value"
+      let (h',v) := interpret h globals locals e in
+      match v with
+      | Thunk ptr => let arr := deref h' ptr in 
+                     let lazy := PArray.get arr (Int63.of_Z 0) in
+                     if is_not_evaluated lazy
+                     then 
+                        match PArray.get arr (Int63.of_Z 1) with 
+                          | Lazy (locals , e) => 
+                            let (h'' , v') := interpret h' globals locals e in
+                           (update h'' ptr (PArray.set arr (Int63.of_Z 0) v'), v')
+                          | _ => (h', fail "not a lazy value")
+                        end
+                     else (h', lazy)
+      | _ => (h', fail "not a lazy value")
       end
-  | _ => fail "assert todo"
-end.
+  | _ => (h , fail "assert todo")
+end. 
 
-Definition cond scr case : bool := 
-  (match case, scr with
-    | Tag n, Block (n', _) => Int63.eqb n n'
-    | Deftag, Block _ => true
-    | Intrange (min, max), value_Int (Int, n) => Z.leb (Int63.to_Z min) n && Z.leb n (Int63.to_Z max)
-    | _, _ => false end).
+Definition Forall2Array {A B:Type} (R : A -> B -> Prop) 
+  (l:list A) (a:array B) default := 
+    List.length l = int_to_nat (PArray.length a) /\
+    forall i:int, int_to_nat i < List.length l -> R (nth (int_to_nat i) l default ) a.[i].
 
-Definition find_match := fun ilocals scr => fix find_match x := match x with
-| (cases, e) :: rest =>
-    if List.existsb (cond scr)  cases then
-      interpret ilocals e
+Class CompatiblePtr `{SemanticsSpec.Heap} `{Heap} :=  
+{ R_ptr : SemanticsSpec.pointer -> pointer -> Prop }.
+
+Inductive vrel `{CompatiblePtr} : SemanticsSpec.value -> value -> Prop :=
+  | vBlock : forall tag vals vals', Forall2Array vrel vals vals' (SemanticsSpec.fail "") ->
+      vrel (SemanticsSpec.Block (tag, vals)) (Block (tag, vals'))
+  | vVec : forall ty ptr ptr', R_ptr ptr ptr' -> vrel (SemanticsSpec.Vec (ty, ptr)) (Vec (ty, ptr'))
+  | vBString : forall ty ptr ptr', R_ptr ptr ptr' -> vrel (SemanticsSpec.BString (ty, ptr)) (BString (ty, ptr'))
+  | vFunc : forall x locals locals' e,  
+    (forall x, vrel (locals x) (locals' x)) ->
+    vrel (SemanticsSpec.Func (locals,x,e)) (Func (locals',x,e))
+  | vRClos : forall self mfix mfix' n locals locals',  
+    (forall x, vrel (locals x) (locals' x)) ->
+    (forall n y e,
+      (nth n mfix SemanticsSpec.Bad_recursive_value = SemanticsSpec.RFunc (y, e)) 
+      <-> 
+      (nth n mfix' Bad_recursive_value = RFunc (y, e))) ->
+    (*  (forall h v, interpret h globals (Ident.Map.add x v (add_all mfix E locals') locals') e = f h v) -> *)
+    vrel (SemanticsSpec.RClos (locals,self,mfix,n)) (RClos (locals',self,mfix',n))
+  | vInt : forall ty i , 
+      vrel (SemanticsSpec.value_Int (ty, i)) (value_Int (ty, i))
+  | vFloat : forall f, 
+      vrel (SemanticsSpec.Float f) (Float f)
+  | vThunk : forall ptr ptr', R_ptr ptr ptr' -> 
+      vrel (SemanticsSpec.Thunk ptr) (Interpreter.Thunk ptr')
+  | vLazy : forall e locals locals',  
+    (forall x, vrel (locals x) (locals' x)) ->
+    vrel (SemanticsSpec.Lazy (locals, e)) (Lazy (locals' , e))
+  | vFail : forall s, 
+      vrel (SemanticsSpec.fail s) (Interpreter.fail s)
+  | vNot_evaluated : vrel SemanticsSpec.not_evaluated Interpreter.not_evaluated.
+
+Definition vrel_locals `{CompatiblePtr} 
+  : Ident.Map.t -> Ident.Map.t -> Prop := fun locals ilocals => forall x, vrel (locals x) (ilocals x).
+
+Class CompatibleHeap `{CompatiblePtr} :=  
+  { R_heap : SemanticsSpec.heap -> heap -> Prop;
+    fresh_compat : forall h ptr h' ih, 
+      R_heap h ih -> SemanticsSpec.fresh h ptr h' -> 
+      let (iptr,ih') := fresh ih in R_ptr ptr iptr /\ R_heap h' ih';
+    update_compat : forall default h ih ptr ptr' h' v v', 
+      R_heap h ih -> SemanticsSpec.update h ptr v h' -> 
+      R_ptr ptr ptr' -> Forall2Array vrel v v' default ->
+      let ih' := Interpreter.update ih ptr' v' in R_heap h' ih';
+    deref_compat : forall default h ih ptr ptr' vals, 
+      R_heap h ih -> SemanticsSpec.deref h ptr vals -> 
+      R_ptr ptr ptr' -> 
+      let vals' := Interpreter.deref ih ptr' in 
+      Forall2Array vrel vals vals' default 
+   }.
+
+
+Lemma Forall2_acc_map {S S' A B B'} (R : S -> S' -> Prop) (RB : B -> B' -> Prop)
+        (f : S' -> A -> S' * B') (P : S -> A -> S -> B -> Prop) x x' y l1 l2 :
+  Forall2_acc P x l1 y l2 ->
+  (forall x x' a b y, R x x' -> P x a y b -> let (y' , b') := f x' a in R y y' /\ RB b b') ->
+  R x x' -> 
+  let (y' , l') := map_acc f x' l1 in R y y' /\ Forall2 RB l2 l'.
+Proof.
+  intros H H'. revert x'. induction H; cbn; intros x' Hx; f_equal; eauto.
+  specialize (H' _ _ _ _ _ Hx H). destruct (f _ _ ) as (s',b').
+  destruct H'. specialize (IHForall2_acc _ H1). destruct (map_acc _ _ _).
+  destruct IHForall2_acc. split; eauto.  
+Qed.
+
+Lemma cond_correct  `{CompatiblePtr} 
+  scr scr' x : vrel scr scr' -> 
+  SemanticsSpec.cond scr x = Interpreter.cond scr' x.
+Proof.
+  now destruct x as [ | | [] ]; destruct 1. 
+Qed.
+
+Lemma existsb_ext {A} (f g : A -> bool) l :
+  (forall x, f x = g x) ->
+  existsb f l = existsb g l.
+Proof.
+  intros H; induction l; cbn; congruence.
+Qed.
+
+Lemma find_match_correct `{CompatiblePtr}  scr scr' cases e h iglobals ilocals :
+  vrel scr scr' ->
+  SemanticsSpec.find_match scr cases = Some e ->
+  Interpreter.find_match Interpreter.interpret h iglobals ilocals scr' cases = interpret h iglobals ilocals e.
+Proof.
+  induction cases as [ | a cases IHcases ]; cbn [SemanticsSpec.find_match]; intros rel Eq.
+  - inversion Eq.
+  - destruct a. 
+    cbn [find_match].
+    destruct existsb eqn:E.
+    * inversion Eq. erewrite existsb_ext. 
+      2:{ intros. symmetry. eapply cond_correct. eauto.  }
+      now rewrite E. 
+    * erewrite existsb_ext.
+      2:{ intros. symmetry. eapply cond_correct. eauto. }
+      rewrite E. eauto.
+Qed.
+
+Lemma Array_of_list'_get {A} s l (a : array A) i :
+  i < s + List.length l ->
+  (s + List.length l < Z.to_nat Int63.wB) ->
+  s + List.length l <= int_to_nat (PArray.length a) ->
+  PArray.get (Array_of_List' s l a) (int_of_nat i) =
+    if (i <? s)%nat then
+      a.[int_of_nat i]
     else
-      find_match rest
-| [] => fail "no case matches" end.
+      nth (i - s) l (a.[int_of_nat i]).
+Proof.
+  intros Hl Hs Ha.
+  induction l as [ | ? ? IHl] in s, i, a, Hl, Hs, Ha |- *.
+  - destruct (Nat.ltb_spec i s).
+    + cbn. reflexivity.
+    + cbn. destruct (i - s); reflexivity.
+  - rewrite IHl. 
+    + cbn in Hl. lia.
+    + cbn [Datatypes.length] in Hs. lia.
+    + rewrite PArray.length_set. cbn [Datatypes.length] in Ha. lia.
+    + fold (int_of_nat s). destruct (Nat.ltb_spec i s) as [H | H].
+      * destruct (Nat.ltb_spec i (S s)) as [H0 | H0]; try lia.
+        rewrite get_set_other.
+        -- intros E. eapply (f_equal int_to_nat) in E.
+           rewrite !int_to_of_nat in E.
+           all:assert (H1 : s < Z.to_nat Int63.wB) by lia.
+           all:eapply inj_lt in H1.
+           all:rewrite Z2Nat.id in H1. all:lia. 
+        -- reflexivity.
+      * destruct (Nat.ltb_spec i (S s)); try lia.
+        -- assert (i = s) by lia. subst.
+           rewrite get_set_same.
+           ++ eapply Int63.ltb_spec.
+              1:eapply Z2Nat.inj_lt.
+              1:eapply Int63.to_Z_bounded.
+              1:eapply Int63.to_Z_bounded. 
+              fold (int_to_nat (int_of_nat s)).
+              rewrite int_to_of_nat. 1:lia.
+              unfold int_to_nat in Ha. lia.
+           ++ cbn. destruct s. 1:reflexivity.
+              rewrite Nat.sub_diag. reflexivity.
+        -- cbn. destruct (i - s) as [ | n] eqn:E.
+           ++ lia.
+           ++ assert (H1 : i - S s = n) by lia. rewrite H1.
+              eapply nth_indep.
+              cbn in Hl. lia.
+Qed.
+
+Lemma Array_of_list_get {A} (a : A) l i :
+  (i < Z.to_nat Int63.wB) ->
+  (List.length l < Z.to_nat Int63.wB) ->
+  List.length l <= int_to_nat max_length ->
+  i < List.length l ->
+  (Array_of_list a l).[int_of_nat i] = nth i l a.
+
+Proof.
+  unfold Array_of_list. intros Hs Hl1 Hl Hi.
+  rewrite Array_of_list'_get.
+  + assumption.
+  + lia. 
+  + rewrite PArray.length_make.
+    fold (int_of_nat (Datatypes.length l)).
+    destruct (Int63.lebP (int_of_nat (Datatypes.length l)) max_length) as [ | n ].
+    * rewrite int_to_of_nat.
+      1:eapply Z2Nat.inj_lt. all: lia. 
+    * destruct n.
+      epose proof (int_to_of_nat (Datatypes.length l) _) as H.
+      eapply Z2Nat.inj_le.
+      1:eapply Int63.to_Z_bounded.
+      1:eapply Int63.to_Z_bounded.
+      unfold int_to_nat in H. rewrite H.
+      unfold int_to_nat in Hl. exact Hl.
+      Unshelve. all:lia.
+  + destruct (Nat.ltb_spec i 0); try lia.
+    rewrite Nat.sub_0_r.
+    eapply nth_indep. lia.
+Qed.
+
+
+Lemma Array_of_list_get_again {A : Set} i s (l : list A) a :
+  i >= s + List.length l ->
+  s + List.length l < Z.to_nat Int63.wB ->
+  i < Z.to_nat Int63.wB ->
+  (Array_of_List' s l a).[int_of_nat i]  = PArray.get a (int_of_nat i).
+Proof.
+  induction l as [ | ? l IHl ] in s, i, a |- *; intros Hi Hs Ha.
+  - cbn. reflexivity.
+  - cbn. rewrite IHl. 
+    + cbn in Hi. lia.
+    + cbn [List.length] in Hs. lia. 
+    + cbn [List.length] in Hs. lia.
+    + rewrite get_set_other. 2:reflexivity.
+      fold (int_of_nat s).
+      intros H. eapply (f_equal int_to_nat) in H.
+      rewrite !int_to_of_nat in H.
+      * eapply inj_lt in Hs.
+        rewrite Z2Nat.id in Hs. 1:cbn; lia.
+        rewrite <- Hs.
+        eapply inj_lt. cbn. lia.
+      * eapply inj_lt in Ha.
+        rewrite Z2Nat.id in Ha. 1:cbn; lia.
+        lia.
+      * subst. cbn in Hi. lia.
+Qed.
+
+Axiom todo : forall {A : Type}, A.
+
+Lemma vrel_add `{CompatiblePtr} x v iv locals ilocals : vrel v iv -> vrel_locals locals ilocals -> 
+  vrel_locals (Ident.Map.add x v locals) (Ident.Map.add x iv ilocals).
+Proof.
+  intros Hv Hlocals nm. unfold Ident.Map.add. now destruct Ident.eqb.
+Qed.
+
+Lemma Array_of_list_S A default n a (l:list A) : 
+  n < Datatypes.length l ->
+  S (Datatypes.length l) <= int_to_nat max_length ->
+  (Array_of_list default (a :: l)).[int_of_nat (S n)] = 
+  (Array_of_list default l).[int_of_nat n].
+Proof.
+  intros. 
+  repeat rewrite Array_of_list_get; cbn in *; try lia; eauto.
+Qed. 
+
+Lemma Array_of_list'_length A k (l:list A) a :
+  PArray.length (Array_of_List' k l a) =
+  PArray.length a.
+Proof. 
+  revert k a. induction l; [reflexivity|].
+  intros; cbn. rewrite IHl. now rewrite PArray.length_set.
+Qed.    
+
+Lemma Array_of_list_length A default (l:list A) :
+  Datatypes.length l < int_to_nat max_length -> 
+  int_to_nat (PArray.length (Array_of_list default l)) =
+  List.length l.
+Proof.
+  unfold Array_of_list. rewrite Array_of_list'_length.
+  rewrite PArray.length_make. intro H. 
+  assert (Hl: (int_of_nat (Datatypes.length l) ≤? max_length)%uint63 = true).
+  { apply leb_spec. rewrite Int63.of_Z_spec. rewrite Z.mod_small; [cbn in *; lia |].
+    cbn in *; lia. }
+  rewrite Hl. apply int_to_of_nat. cbn in *; lia. 
+Qed.    
+  
+Lemma Forall2_acc_length {X A B R x l y l'} : @Forall2_acc X A B R x l y l' -> List.length l = List.length l'.
+Proof. 
+  induction 1; cbn; eauto.
+Qed.   
+
+Lemma Forall2_length {A B P l l'} : @Forall2 A B P l l' -> List.length l = List.length l'.
+Proof. 
+  induction 1; cbn; eauto.
+Qed.
+
+Lemma isNotEvaluated_vrel `{CompatiblePtr} v v' b : 
+  vrel v v' -> isNotEvaluated v = b <-> is_not_evaluated v' = b.
+Proof.
+  now destruct 1.
+Qed.    
+
+Axiom funext : forall A B, forall f g : A -> B, (forall x, f x = g x) -> f = g.
+
+Lemma interpret_ilocals_proper `{CompatiblePtr} ih iglobals ilocals ilocals' e :
+  (forall x, ilocals x = ilocals' x) ->
+  interpret ih iglobals ilocals e = interpret ih iglobals ilocals' e.
+Proof.
+  intros Hlocal; apply funext in Hlocal. now subst.
+Qed.  
+  
+Ltac fail_case IHeval Hloc Hheap Heq := 
+  let Hv := fresh "iv1" in cbn; specialize (IHeval _ _ Hloc Hheap); destruct interpret as [? ?];
+  destruct IHeval as [? Hv]; destruct Hv; inversion Heq; split;eauto; econstructor.
+
+Lemma vrel_loacs_add_self `{CompatiblePtr}  locals' locals'0 mfix mfix' self :
+  (forall x : Ident.t, vrel (locals' x) (locals'0 x)) ->
+  (forall (n : nat) (y : Ident.t) (e : t),
+     nth n mfix SemanticsSpec.Bad_recursive_value = SemanticsSpec.RFunc (y, e) <->
+    nth n mfix' Bad_recursive_value = RFunc (y, e)) ->
+  vrel_locals (SemanticsSpec.add_self self mfix locals') (add_self self mfix' locals'0).
+Proof. 
+  intros Hloc ?.
+  unfold add_self, SemanticsSpec.add_self.
+  unfold add_recs, SemanticsSpec.add_recs. unfold mapi.
+  generalize 0. generalize self at 1 3. 
+  pose proof (Hcopy := Hloc). revert Hcopy.  
+  generalize locals' at 1 3. generalize locals'0 at 1 3.
+  revert locals' locals'0 Hloc.     
+  induction self; cbn; eauto; intros. apply IHself; eauto. 
+  intro. unfold Ident.Map.add. case_eq (Ident.eqb x a); intro; eauto. 
+  now econstructor.
+Qed. 
+
+
+Lemma eval_correct `{CompatibleHeap} 
+  globals locals ilocals iglobals e h h' ih v :
+  (forall nm val, In (nm, val) globals -> vrel val (iglobals nm)) ->
+  vrel_locals locals ilocals ->
+  R_heap h ih ->
+  eval _ globals locals h e h' v -> 
+  let (ih',iv) := interpret ih iglobals ilocals e in R_heap h' ih' /\ vrel v iv.  
+Proof.
+  rename H into _Heap; rename H0 into _iHeap; rename H1 into _CPtr; rename H2 into _CHeap. 
+  intros Hglob Hloc Hheap.
+  induction 1 as [ (* lambda_sing *) locals h x e
+                 | (* lambda *) locals h x ids e H
+                 | (* app_sing *) locals h1 h2 h3 h4 x locals' e e2 v2 e1 v H IHeval1 H0 IHeval2 H1 IHeval3
+                 | (* app_sing_Rec *) locals h1 h2 h3 h4 mfix n y e locals' self e2 v2 e1 v H IHeval1 H0 IHeval2 Hnth H1 IHeval3
+                 | (* app_fail *) locals h h' e2 e v Heval IHeval Heq
+                 | (* app *) locals h h' e2 e1 v vals tag IHeval 
+                 | (* var *) 
+                 | (* let_body *) | (* let_unnamed *) | (* let_named *) | (* let_rec *)
+                 | (* switch *) 
+                 | (* block *)  
+                 | (* field *) locals h h' idx b vals tag H IHeval | | | | | | 
+                 | | | | | | | | | | | | | | | | | | | ]
+                 in ih, Hheap, ilocals, Hloc |- *. 
+  (* eval_lambda_sing *) 
+  - split; eauto. econstructor; eauto.
+  (* eval_lambda *)
+  - split; eauto. 
+    destruct ids as [ | t ids ]; cbn in H. 1:inversion H. clear H.
+    econstructor; eauto.  
+  (* eval_app_sing *)
+  - cbn; specialize (IHeval1 _ _ Hloc Hheap). destruct interpret as [ih1 iv1]; destruct IHeval1 as [Hheap1  Hiv1].
+    specialize (IHeval2 _ _ Hloc Hheap1). destruct interpret as [ih2 iv2]; destruct IHeval2 as [Hheap2  Hiv2].
+    inversion Hiv1 ; subst.
+    specialize (IHeval3 (Ident.Map.add x iv2 locals'0) ih2). 
+    destruct interpret as [ih3 iv3]; cbn in *.
+    apply IHeval3; eauto. now apply vrel_add. 
+  (* eval_app_sing_rec *)
+  - cbn; specialize (IHeval1 _ _ Hloc Hheap). destruct interpret as [ih1 iv1]; destruct IHeval1 as [Hheap1  Hiv1].
+    specialize (IHeval2 _ _ Hloc Hheap1). destruct interpret as [ih2 iv2]; destruct IHeval2 as [Hheap2  Hiv2].
+    inversion Hiv1 ; subst.
+    edestruct H8. specialize (H2 Hnth). rewrite H2.
+    specialize (IHeval3 (Ident.Map.add y iv2 (add_self self mfix' locals'0)) ih2). 
+    destruct interpret as [ih3 iv3]; cbn in *.
+    apply IHeval3; eauto. apply vrel_add; eauto.
+    now apply vrel_loacs_add_self. 
+  (* eval_app_fail *)
+  - fail_case IHeval Hloc Hheap Heq.
+  (* eval_app *)
+  - now apply IHeval.
+  (* eval_var *)
+  - cbn; eauto.
+  (* eval_let_body *)
+  - now eapply IHeval.
+  (* eval_let_unnamed *)
+  - cbn; specialize (IHeval1 _ _ Hloc Hheap). destruct interpret as [ih1 iv1]; destruct IHeval1 as [Hheap1  Hiv1].
+    now eapply IHeval2. 
+  (* eval_let_named *)
+  - cbn; specialize (IHeval1 _ _ Hloc Hheap). destruct interpret as [ih1 iv1]; destruct IHeval1 as [Hheap1  Hiv1].
+    eapply IHeval2; eauto. now apply vrel_add. 
+  (* eval_let_rec *)
+  - cbn; eapply IHeval; eauto. intros x. clear IHeval. subst.
+    apply vrel_loacs_add_self; eauto.
+    intros. unfold rfunc. set (l := map snd recs). clearbody self l. split. 
+    + revert n. induction l; cbn.
+      * intros n H; destruct n; eauto; cbn in *; inversion H.
+      * intros n H. destruct n; eauto. 
+        destruct a; inversion H. destruct p. destruct l0 ; inversion H.
+        destruct l0 ; now inversion H. 
+    + revert n. induction l; cbn.
+      * intros n H; destruct n; eauto; cbn in *; inversion H.
+      * intros n H. destruct n; eauto. 
+        destruct a; inversion H. destruct p. destruct l0 ; inversion H.
+        destruct l0 ; now inversion H. 
+  (* eval_switch *)
+  - cbn.
+    specialize (IHeval1 _ _ Hloc Hheap). destruct interpret as [ih1 iv1]; destruct IHeval1 as [Hheap1  Hiv1].
+    erewrite find_match_correct; eauto. now apply IHeval2.
+  (* eval_block *)
+  - cbn. clear H. revert ih Hheap. induction H1. 
+    + intros ih Hheap. split ; eauto. econstructor.
+      split; [ reflexivity|]. cbn. lia.
+    + intros ih Hheap. simpl. 
+      specialize (H _ _ Hloc Hheap). destruct interpret as [ih1 iv1]; destruct H as [Hheap1  Hiv1]. 
+      assert (Hlength: Datatypes.length l' < int_to_nat max_length) by (cbn in *; lia). 
+      specialize (IHForall2_acc Hlength ih1 Hheap1).     
+      unshelve epose proof (Forall2_acc_map R_heap vrel
+        (fun (h : Interpreter.heap) (e : t) => interpret h iglobals ilocals e) _ _ _ _ _ _ H1 _ Hheap1).
+      { clear -Hloc. intros. cbn in *. specialize (H0 ilocals x'). destruct interpret. apply H0; eauto. }
+      set (p := map_acc _ ih1 l) in *. destruct p. destruct H as [Heahp2 Hl0]. split; eauto. 
+      destruct IHForall2_acc as [? IHForall2_acc]. 
+      assert (Hl: (int_of_nat (Datatypes.length l) ≤? max_length)%uint63 = true).
+      { apply leb_spec. rewrite Int63.of_Z_spec.
+        rewrite (Forall2_acc_length H1). rewrite Z.mod_small; [cbn in *; lia |]. cbn in *; lia. } 
+      assert (Hl': (int_of_nat (S (Datatypes.length l)) ≤? max_length)%uint63 = true).
+      { apply leb_spec. rewrite Int63.of_Z_spec. rewrite (Forall2_acc_length H1). rewrite Z.mod_small; [cbn in *; lia |].
+        cbn in *; lia. } 
+      rewrite Hl in IHForall2_acc. rewrite Hl'. inversion IHForall2_acc; subst. clear IHForall2_acc.  
+      econstructor. destruct H3. split.
+      * simpl. rewrite Array_of_list_length.
+        { cbn. rewrite <- (Forall2_length Hl0). clear - H0; cbn in *; lia. }
+        now rewrite (Forall2_length Hl0).
+      * intros idx Hidx. rewrite <- (int_of_to_nat idx) at 2.
+        pose proof (Hbounded := to_Z_bounded idx).
+        destruct (int_to_nat idx).
+        ** simpl. pose Int63.wB_pos. rewrite Array_of_list_get; try (cbn; lia).
+          ++ cbn in H0. rewrite (Forall2_length Hl0) in H0. clear - H0; cbn in *; lia. 
+          ++ cbn in H0. rewrite (Forall2_length Hl0) in H0. clear - H0; cbn in *; lia. 
+          ++ eauto.
+        ** simpl. rewrite Array_of_list_S. 
+           ++ cbn; cbn in Hidx. rewrite <- (Forall2_length Hl0). lia.
+           ++ cbn; cbn in H0. rewrite <- (Forall2_length Hl0). lia.
+           ++ specialize (H3 (int_of_nat n)). 
+              rewrite int_to_of_nat in H3.
+              { cbn; cbn in Hidx; cbn in H0. lia. }
+              eapply H3. cbn in Hidx; lia.  
+  (* eval_field *)    
+  - cbn. specialize (IHeval _ _ Hloc Hheap). destruct interpret as [ih1 iv1]; destruct IHeval as [Hheap1  Hiv1].
+    split; eauto. inversion Hiv1; subst. clear Hiv1. destruct H6 as [? H5]. 
+    now eapply (H5 idx).  
+  (* eval_field_fail *)    
+  - fail_case IHeval Hloc Hheap H0.
+  (* eval_lazy *)  
+  - cbn. pose proof (fresh_compat _ _ _ _ Hheap H).
+    set (Interpreter.fresh ih) in *. destruct p.
+    destruct H1; split; [| now econstructor].
+    eapply update_compat with (default := SemanticsSpec.fail ""); eauto. 
+    split; [reflexivity|].
+    intros idx Hidx. rewrite <- (int_of_to_nat idx). destruct int_to_nat. 
+    * cbn. econstructor; eauto.
+    * cbn in Hidx. destruct n; [compute|lia].
+      econstructor; eauto.
+  (* eval_force_done *)  
+  - cbn. specialize (IHeval _ _ Hloc Hheap). destruct interpret as [ih1 iv1]; destruct IHeval as [Hheap1  Hiv1]. 
+    inversion Hiv1; subst; clear Hiv1.
+    pose proof (deref_compat (SemanticsSpec.fail "") _ _ _ _ _ Hheap1 H0 H5).
+    destruct H2 as [? Hderef]. pose proof (Hderef (int_of_nat 0)).
+    cbn in H4. rewrite isNotEvaluated_vrel in H3; eauto.
+    + eapply H4. lia.
+    + destruct is_not_evaluated; inversion H3.
+      split; eauto. eapply H4. lia.
+  (* eval_force *)  
+  - cbn; specialize (IHeval1 _ _ Hloc Hheap). destruct interpret as [ih1 iv1]; destruct IHeval1 as [Hheap1  Hiv1].
+    inversion Hiv1; subst; clear Hiv1.
+    pose proof (deref_compat (SemanticsSpec.fail "") _ _ _ _ _ Hheap1 H0 H7).
+    destruct H6 as [? Hderef]. pose proof (Hderef (int_of_nat 0)).
+    cbn in H8. rewrite isNotEvaluated_vrel in H2; [eapply H8; lia|]. 
+    destruct is_not_evaluated; inversion H2. clear H2. 
+    rewrite H1 in Hderef. 
+    specialize (Hderef (int_of_nat 1) (ltac:(eauto))).
+    rewrite H3 in Hderef. cbn in Hderef. set _.[1] in *. 
+    inversion Hderef. subst. rewrite <- H11 in Hderef.
+    specialize (IHeval2 _ _ H9 Hheap1). 
+    destruct interpret as [ih2 iv2]; destruct IHeval2 as [Hheap2  Hiv2].
+    split; eauto. 
+    eapply update_compat with (default := SemanticsSpec.fail ""); eauto. split; cbn.   
+    * rewrite PArray.length_set. lia.
+    * intro i. pose proof (int_of_to_nat i). destruct (int_to_nat i); [| destruct  n].
+      + subst. intros _. rewrite get_set_same; eauto.
+        rewrite <- (int_of_to_nat (PArray.length _)). rewrite <- H6. 
+        rewrite H1. cbn; lia.
+      + subst; intros _. rewrite get_set_other; [now apply eqb_false_spec|]. cbn.
+        fold y. rewrite <- H11. econstructor; eauto.
+      + lia. 
+  (* eval_force_fail *)  
+  - fail_case IHeval Hloc Hheap H0.
+  (* eval_global *)  
+  - cbn. split; eauto. 
+  - 
+  Qed.
+Set Guard Checking.
+
+
+(*  Lemma vtrans_inj v v' : vtrans v = vtrans v' -> v = v'.
+  Admitted. 
+  Lemma apD {A B} {f g : forall a:A, B a} : f = g -> forall x, f x = g x. 
+  now destruct 1.
+  Defined.  *)
+
+  Lemma interp_correct iglobals globals locals e v ilocals :
+    (forall x, vrel iglobals (ilocals x) (locals x)) ->
+    vrel (interpret ilocals e) v -> eval globals locals e v.
+  induction e; intro Hlocal; cbn in *. 
+  - intros Hvar. unfold Ident.Map.find in Hvar. rewrite Hlocal in Hvar.
+    apply vtrans_inj in Hvar. subst. econstructor. 
+  - intros Hlambda. destruct p as [xs e]. induction xs; cbn in *.
+    * admit.
+    * destruct xs.
+      + destruct v; cbn in Hlambda; try destruct p; try now inversion Hlambda.
+        destruct p. inversion Hlambda. clear Hlambda.
+        pose proof (Hlambda := apD H0 a). 
+        
+         H0. pose (ap )
+        f_equal
+        
+        eapply eval_lambda_sing. 
+           
+
+  destruct v. inversion Hvar.  eapply eval_var. 
 
