theories/SemanticsSpec.v
@@ -1,9 +1,36 @@
+
 Require Import ssreflect.
-From Malfunction Require Import Malfunction Interpreter.
+From Malfunction Require Import Malfunction.
+From MetaCoq.PCUIC Require Import PCUICAst PCUICFirstorder.
 
 Require Import ZArith Array.PArray List String Floats Lia.
 From MetaCoq Require Import bytestring.
 Import ListNotations.
+
+Definition int_to_nat (i : int) : nat :=
+  Z.to_nat (Int63.to_Z i).
+
+Definition int_of_nat n := Uint63.of_Z (Coq.ZArith.BinInt.Z.of_nat n).
+
+Lemma int_of_to_nat i :
+  int_of_nat (int_to_nat i) = i.
+Proof.
+  unfold int_of_nat, int_to_nat.
+  rewrite Z2Nat.id.
+  1:eapply Int63.to_Z_bounded.
+  now rewrite Int63.of_to_Z.
+Qed.
+
+Lemma int_to_of_nat i :
+  (Z.of_nat i < Int63.wB)%Z ->
+  int_to_nat (int_of_nat i) = i.
+Proof.
+  unfold int_of_nat, int_to_nat.
+  intros ?.
+  rewrite Int63.of_Z_spec.
+  rewrite Z.mod_small. 1:lia.
+  now rewrite Nat2Z.id.
+Qed.
 
 Set Default Goal Selector "!".
 
@@ -44,9 +71,6 @@ Inductive value `{Heap} :=
 
 Definition heap `{Heap} := heapGen value.
 
-(* Class CompatiblePtr `{Heap} `{Interpreter.Heap} :=  
-{ R_ptr : pointer -> Interpreter.pointer -> Prop }. *)
-
  From Coq Require Import Uint63.
 
  Definition list_of_array {A : Type} (a:array A) : list A :=
@@ -82,9 +106,52 @@ Definition isNotEvaluated `{Heap} (s : value) : bool :=
   | _ => false
   end.  
 
-Definition int_to_nat (i : int) : nat :=
-  Z.to_nat (Int63.to_Z i).
+Definition fail_def {A} (a : A) (s : string) : A.
+  exact a.
+Qed.
 
+Definition fail_float := fail_def infinity.
+Definition fail_Z := fail_def Z.zero.
+
+Definition bitwidth := fun t =>
+match t with
+| Int => 63
+| Int32 => 32
+| Int64 => 64
+| BigInt => fail_Z "no bitwidth for bigint"
+end%Z.
+
+Definition truncate `{Heap} ty n :=
+  value_Int (ty, match ty with
+                 | Bigint => n
+                 | ty =>
+                     let width := bitwidth ty in
+                     let range := Z.shiftl (Z.of_nat 1) width in
+                     let masked := Z.land n (Z.sub range (Z.of_nat 1)) in
+                     let min_int := Z.shiftr range 1 in
+                     if Z.ltb masked min_int then masked else
+                       Z.sub masked range
+                 end). 
+
+Definition inttype_eqb (t1 t2 : inttype) :=
+  match t1, t2 with
+  | Int, Int
+  | Int32, Int32
+  | Int64, Int64
+  | Bigint, Bigint => true
+  | _, _ => false
+  end.
+
+Definition as_ty `{Heap} ty := fun ty2 =>
+  match ty2 with
+  | value_Int (ty', n) => if inttype_eqb ty ty' then n else fail_Z "integer type missmatch"
+  | _ => fail_Z "expected integer"
+  end.
+
+Definition as_float `{Heap} x := match x with
+  | Float f => f
+  | _ => fail_float "expected float64"
+end.
 
 Definition cond `{Heap} scr case : bool := 
   (match case, scr with
@@ -113,6 +180,15 @@ Fixpoint mapi_ {A B} (f : nat -> A -> B) (l : list A) (n:nat) : list B :=
 
 Definition mapi {A B} (f : nat -> A -> B) l := mapi_ f l 0. 
 
+Definition init {A} (size : nat) (f : nat -> A) : list A := map f (seq 0 size).
+
+Fixpoint set {A} (l : list A) (n : nat) (a:A) : list A 
+  := match l , n with
+    [] , _ =>  []
+  | x :: l , 0 => a :: l
+  | x :: l , S n => x :: set l n a
+  end.
+
 Definition RFunc_build `{Heap} recs := 
     map (fun t =>
       match t with 
@@ -130,17 +206,58 @@ Definition add_self `{Heap} self rfunc locals :=
   List.fold_right (fun '(x,t) l => Ident.Map.add x t l) locals (add_recs locals self rfunc) .
   (*   List.fold_right (fun '(x,t) l => Ident.Map.add x t l) locals (add_recs locals self rfunc). *)
 
-Definition Forall2Array {A B:Type} (R : A -> B -> Prop) 
-  (l:list A) (a:array B) default := 
-    List.length l = int_to_nat (PArray.length a) /\
-    forall i:int, int_to_nat i < List.length l -> R (nth (int_to_nat i) l default ) a.[i].
-
 Inductive
   Forall2_acc {X A B : Type} (R : X -> A -> X -> B -> Prop) : X -> list A -> X -> list B -> Prop :=
     Forall2_acc_nil : forall x, Forall2_acc R x [] x []
     | Forall2_acc_cons : forall (x y z : X) (a : A) (b : B) 
                             (l : list A) (l' : list B) ,
                      R x a y b -> Forall2_acc R y l z l' -> Forall2_acc R x (a :: l) z (b :: l').
+
+Definition comparison_eqb x1 x2 :=
+  match x1, x2 with
+  | Datatypes.Lt, Datatypes.Lt | Datatypes.Gt, Datatypes.Gt | Datatypes.Eq, Datatypes.Eq => true
+  | _, _ => false
+  end.
+
+Definition binary_comparison_eqb op cmp := 
+  match op with
+  | Lt => comparison_eqb cmp Datatypes.Lt
+  | Gt => comparison_eqb cmp Datatypes.Gt
+  | Lte => negb (comparison_eqb cmp Datatypes.Gt)
+  | Gte => negb (comparison_eqb cmp Datatypes.Lt)
+  | Eq => comparison_eqb cmp Datatypes.Eq
+  end.
+
+Definition binary_op_to_float op v1 v2 : float := 
+  match op with
+   | Sub => v1 - v2
+   | Mul => v1 * v2
+   | Div => v1 / v2
+   | Mod => fail_float "mod on floats not supported" 
+   | Add => v1 + v2 
+  end.
+
+Definition binary_comparison_to_bool op e1 e2 :=
+  match op with
+  | Lt => PrimFloat.ltb e1 e2
+  | Gt => PrimFloat.ltb e2 e2
+  | Lte => PrimFloat.leb e1 e2
+  | Gte => PrimFloat.leb e2 e1
+  | Eq => PrimFloat.eqb e1 e2
+  end.
+
+Definition option_def {A} (a : A) (x : option A) : A :=
+  match x with
+  | None => a
+  | Some a => a
+  end.
+
+Definition vector_type_eqb (t1 t2 : vector_type) :=
+  match t1, t2 with
+  | Array, Array
+  | Bytevec, Bytevec => true
+  | _, _ => false
+  end.
 
 Section eval.
 
@@ -216,7 +333,7 @@ Inductive eval (locals : @Ident.Map.t value) : heap -> t -> heap -> value -> Pro
 | eval_force_done h h' e ptr vals lazy :
   eval locals h e h' (Thunk ptr) ->
   deref h' ptr vals ->
-  List.length vals > 0 -> 
+  List.length vals > 1 -> 
   nth 0 vals (fail "") = lazy ->
   isNotEvaluated lazy = false ->
   eval locals h (Mforce e) h' lazy 
@@ -235,7 +352,147 @@ Inductive eval (locals : @Ident.Map.t value) : heap -> t -> heap -> value -> Pro
   eval locals h (Mforce e) h' (fail "not a lazy value")
 | eval_global h nm v :
   In (nm, v) globals ->
-  eval locals h (Mglobal nm) h v.
+  eval locals h (Mglobal nm) h v
+| eval_num_int n h : eval locals h (Mnum (numconst_Int n)) h (value_Int (Int, Int63.to_Z n))
+| eval_num_bigint n h : eval locals h (Mnum (numconst_Bigint n)) h  (value_Int (Bigint, n))
+| eval_num_float f h : eval locals h (Mnum (numconst_Float64 f)) h  (Float f)
+| eval_string s h h' h'' ptr : 
+  let str := init (length s)
+    (fun i => value_Int (Int, Z.of_nat (Ascii.nat_of_ascii (option_def Ascii.Space (String.get i s))))) in
+  fresh h ptr h' -> 
+  update h' ptr str h'' ->
+  eval locals h (Mstring s) h'' (Vec (Bytevec, ptr))
+| eval_numop1 op ty e h h' v : 
+   eval locals h e h' v -> 
+   let n := as_ty ty v in
+   eval locals h (Mnumop1 (op, embed_inttype ty, e)) h' (truncate ty (match op with Malfunction.Neg => Z.mul (-1) n | Not => Z.lnot n end))
+| eval_numop2 op ty e1 e2 v1 v2 h h1 h2 :
+      eval locals h e1 h1 v1 ->
+      eval locals h1 e2 h2 v2 ->
+      eval locals h (Mnumop2 (op, embed_inttype ty, e1, e2)) h2  
+      match op with
+      | embed_binary_arith_op op =>
+          let f := match op with
+                   | Sub => Z.sub | Mul => Z.mul | Div => Z.div | Mod => Z.rem | Add => Z.add 
+                   end in
+          truncate ty (f (as_ty ty v1) (as_ty ty v2))
+      | embed_binary_bitwise_op op =>
+          let n := as_ty ty v1 in
+          let c := as_ty Int v2 in
+          (* TODO is this test necessary? *)
+          truncate ty (match op with
+          | And => Z.land (as_ty ty v1) (as_ty ty v2)
+          | Or => Z.lor (as_ty ty v1) (as_ty ty v2)
+          | Xor => Z.lxor (as_ty ty v1) (as_ty ty v2)
+          | Lsl => Z.shiftl n c
+          | Asr => Z.shiftr n c
+          | Lsr => 
+              let n := match ty with
+                       | Bigint => n
+                       | _ =>
+                           let w := bitwidth ty in
+                           Z.land n (Z.sub (Z.shiftl (Z.of_nat 1) w) (Z.of_nat 1)) end in
+              Z.shiftr n c end)
+      | embed_binary_comparison op =>
+          let cmp := Z.compare (as_ty ty v1) (as_ty ty v2) in
+          let res := binary_comparison_eqb op cmp in
+          value_Int (Int, if res then 1%Z else 0%Z)
+      end
+| eval_numop1_neg e h h' v :  
+    eval locals h e h' v ->
+    eval locals h (Mnumop1 (Malfunction.Neg, Float64, e)) h' (Float (- as_float v))
+| eval_numop1_float_fail h x : 
+  eval locals h (Mnumop1 (Not, Float64, x)) 
+              h (fail "invalid bitwise float operation")
+| eval_numop2_float_fail h x y n : 
+    eval locals h (Mnumop2 (embed_binary_bitwise_op n, Float64, x, y)) 
+                h (fail "invalid bitwise float operation")
+| eval_numop2_float h h1 h2 op e1 e2 v1 v2 :
+      eval locals h e1 h1 v1 ->
+      eval locals h1 e2 h2 v2 ->
+      let v1' := as_float v1 in
+      let v2' := as_float v2 in
+      eval locals h (Mnumop2 (embed_binary_arith_op op, Float64, e1, e2))
+                  h2 (Float (binary_op_to_float op v1' v2'))
+| eval_numop2_embed_float h h1 h2 op e1 e2 v1 v2 :
+      eval locals h e1 h1 v1 ->
+      eval locals h1 e2 h2 v2 ->
+      let v1' := as_float v1 in
+      let v2' := as_float v2 in
+      let res := binary_comparison_to_bool op v1' v2' in
+      eval locals h (Mnumop2 (embed_binary_comparison op, Float64, e1, e2))
+                  h2 (value_Int (Int, if res then 1%Z else 0%Z))
+| eval_convert_int h h' e v src dst : 
+      eval locals h e h' v ->
+      eval locals h (Mconvert (embed_inttype src, embed_inttype dst, e))
+                  h' (truncate dst (as_ty src v))
+| eval_convert_float h h' e v src :
+      eval locals h e h' v ->
+      eval locals h (Mconvert (embed_inttype src, Float64, e))
+                  h' (Float (PrimFloat.of_uint63 (Int63.of_Z (as_ty src v))))
+| eval_convert_float_float h h' v e :
+      eval locals h e h' v ->
+      eval locals h (Mconvert (Float64, Float64, e)) 
+                  h' (Float (as_float v))                                              
+| eval_vecnew_array h h1 h2 h3 h4 len len' def def' ptr : 
+      eval locals h len h1 (value_Int (Int, len')) -> 
+      eval locals h1 def h2 def' ->
+      fresh h2 ptr h3 -> 
+      update h3 ptr (init (Z.to_nat len') (fun _ => def')) h4 ->
+      eval locals h (Mvecnew (Array, len, def)) h4 (Vec (Array, ptr))
+| eval_vecnew_bytevec h h1 h2 h3 h4 len len' def k ptr : 
+      eval locals h len h1 (value_Int (Int, len')) -> 
+      eval locals h1 def h2 (value_Int (Int, k)) ->
+      fresh h2 ptr h3 -> 
+      update h3 ptr (init (Z.to_nat len') (fun _ => (value_Int (Int, k)))) h4 ->
+      eval locals h (Mvecnew (Bytevec, len, def)) 
+                  h4 (if Z.leb 0%Z k && Z.ltb k 256 
+                      then Vec (Bytevec, ptr)
+                      else fail "bad vector creation")
+| eval_vecget h h1 h2 vec ty' idx idx' ty ptr arr : 
+    eval locals h vec h1 (Vec (ty', ptr)) -> 
+    eval locals h1 idx h2 idx' ->
+    deref h ptr arr ->
+    eval locals h (Mvecget (ty, vec, idx)) 
+                h2 (match idx' with
+       | value_Int (Int,i) =>
+           if vector_type_eqb ty ty' then
+             if Z.leb 0 i && Z.ltb i (Z.of_nat (List.length arr)) then
+               nth (Z.to_nat i) arr (fail "")
+             else
+               fail "index out of bounds: %d"
+           else
+             fail "wrong vector type"
+       | _ => fail "wrong vector type"
+       end)
+  | eval_vecset h h1 h2 h3 h4 vec ty ty' ptr idx i e v arr :  
+  eval locals h vec h1 (Vec (ty', ptr)) -> 
+  eval locals h1 idx h2 (value_Int (Int, i)) ->
+  eval locals h2 e h3 v ->
+  deref h ptr arr -> 
+  update h3 ptr (set arr (Z.to_nat i) v) h4 ->
+  eval locals h (Mvecset (ty, vec, idx, e)) 
+              h4 (if vector_type_eqb ty ty' then 
+        let i := Int63.of_Z i in 
+        if Int63.leb (int_of_nat 0) i && Int63.leb i (int_of_nat (List.length arr)) then 
+          match ty, v with 
+          | Array, _ => value_Int (Int, 0%Z)
+          | Bytevec, value_Int (Int, val) => 
+            if (Z.leb 0 val) && (Z.ltb val 256)
+            then 
+              value_Int (Int, 0%Z)
+            else fail "not a byte"
+          | Bytevec, _ => fail "not a byte"
+          end 
+        else fail "index out of bounds: %d"
+    else fail "wrong vector type")  
+| eval_veclen h h' vec ty' ptr ty arr : 
+  eval locals h vec h' (Vec (ty', ptr)) -> 
+  deref h ptr arr -> 
+  eval locals h (Mveclen (ty, vec)) 
+              h' (if vector_type_eqb ty ty' then value_Int (Int, Z.of_nat (List.length arr))
+                                    else fail "wrong vector type")
+.
 
 Lemma eval_ind :
 forall P : Ident.Map.t -> heap -> t -> heap -> value -> Prop,
@@ -258,15 +515,15 @@ forall P : Ident.Map.t -> heap -> t -> heap -> value -> Prop,
         P locals h (Mapply (e1, [e2])) h3 v) ->
        (forall (locals : Ident.Map.t) (h h1 h2 h3 : heap)
           (mfix : list rec_value) (n : nat) (y : Ident.t) 
-          (e : t) (locals' locals'' : Ident.Map.t) self
+          (e : t) (locals'  : Ident.Map.t) self
           (e2 : t) (v2 : value) (e1 : t) (v : value),
         eval locals h e1 h1 (RClos (locals', self, mfix, n)) ->
         P locals h e1 h1 (RClos (locals', self, mfix, n)) ->
         eval locals h1 e2 h2 v2 ->
         P locals h1 e2 h2 v2 ->
         nth n mfix Bad_recursive_value = RFunc (y, e) ->
-        eval (Ident.Map.add y v2 locals'') h2 e h3 v ->
-        P (Ident.Map.add y v2 locals'') h2 e h3 v ->
+        eval (Ident.Map.add y v2 (add_self self mfix locals')) h2 e h3 v ->
+        P (Ident.Map.add y v2 (add_self self mfix locals')) h2 e h3 v ->
         P locals h (Mapply (e1, [e2])) h3 v) ->
        (forall (locals : Ident.Map.t) (h h1 : heap) (e2 e1 : t) (v : value),
         eval locals h e1 h1 v ->
@@ -351,7 +608,7 @@ forall P : Ident.Map.t -> heap -> t -> heap -> value -> Prop,
         eval locals h e h' (Thunk ptr) ->
         P locals h e h' (Thunk ptr) ->
         deref h' ptr vals ->
-        Datatypes.length vals > 0 ->
+        Datatypes.length vals > 1 ->
         nth 0 vals (fail "") = lazy ->
         isNotEvaluated lazy = false -> P locals h (Mforce e) h' lazy) ->
        (forall (locals : Ident.Map.t) (h h' h'' : heap)
@@ -374,539 +631,228 @@ forall P : Ident.Map.t -> heap -> t -> heap -> value -> Prop,
         P locals h (Mforce e) h' (fail "not a lazy value")) ->
        (forall (locals : Ident.Map.t) (h : heap) (nm : Ident.t) (v : value),
         In (nm, v) globals -> P locals h (Mglobal nm) h v) ->
-       forall (locals : Ident.Map.t) (h : heap) (t : t) 
+       (forall (locals : Ident.Map.t) (n : Malfunction.int) (h : heap),
+        P locals h (Mnum (numconst_Int n)) h (value_Int (Int, φ (n)%uint63))) ->
+       (forall (locals : Ident.Map.t) (n : Z) (h : heap),
+        P locals h (Mnum (numconst_Bigint n)) h (value_Int (Bigint, n))) ->
+       (forall (locals : Ident.Map.t) (f21 : float) (h : heap),
+        P locals h (Mnum (numconst_Float64 f21)) h (Float f21)) ->
+       (forall (locals : Ident.Map.t) (s : string) 
+          (h h' h'' : heapGen value) (ptr : pointer),
+        let str :=
+          init (length s)
+            (fun i : nat =>
+             value_Int
+               (Int,
+                Z.of_nat
+                  (Ascii.nat_of_ascii (option_def Ascii.Space (get i s)))))
+          in
+        fresh h ptr h' ->
+        update h' ptr str h'' ->
+        P locals h (Mstring s) h'' (Vec (Bytevec, ptr))) ->
+       (forall (locals : Ident.Map.t) (op : unary_num_op) 
+          (ty : inttype) (e : t) (h h' : heap) (v : value),
+        eval locals h e h' v ->
+        P locals h e h' v ->
+        let n := as_ty ty v in
+        P locals h (Mnumop1 (op, embed_inttype ty, e)) h'
+          (truncate ty
+             match op with
+             | Malfunction.Neg => -1 * n
+             | Not => Z.lnot n
+             end)) ->
+       (forall (locals : Ident.Map.t) (op : binary_num_op) 
+          (ty : inttype) (e1 e2 : t) (v1 v2 : value) 
+          (h h1 h2 : heap),
+        eval locals h e1 h1 v1 ->
+        P locals h e1 h1 v1 ->
+        eval locals h1 e2 h2 v2 ->
+        P locals h1 e2 h2 v2 ->
+        P locals h (Mnumop2 (op, embed_inttype ty, e1, e2)) h2
+          match op with
+          | embed_binary_arith_op op0 =>
+              let f24 :=
+                match op0 with
+                | Malfunction.Add => Z.add
+                | Sub => Z.sub
+                | Mul => Z.mul
+                | Div => Z.div
+                | Mod => Z.rem
+                end in
+              truncate ty (f24 (as_ty ty v1) (as_ty ty v2))
+          | embed_binary_bitwise_op op0 =>
+              let n := as_ty ty v1 in
+              let c := as_ty Int v2 in
+              truncate ty
+                match op0 with
+                | And => Z.land (as_ty ty v1) (as_ty ty v2)
+                | Or => Z.lor (as_ty ty v1) (as_ty ty v2)
+                | Xor => Z.lxor (as_ty ty v1) (as_ty ty v2)
+                | Lsl => Z.shiftl n c
+                | Lsr =>
+                    let n0 :=
+                      match ty with
+                      | Bigint => n
+                      | _ =>
+                          let w := bitwidth ty in
+                          Z.land n (Z.shiftl (Z.of_nat 1) w - Z.of_nat 1)
+                      end in
+                    Z.shiftr n0 c
+                | Asr => Z.shiftr n c
+                end
+          | embed_binary_comparison op0 =>
+              let cmp := (as_ty ty v1 ?= as_ty ty v2)%Z in
+              let res := binary_comparison_eqb op0 cmp in
+              value_Int (Int, if res then 1%Z else 0%Z)
+          end) ->
+       (forall (locals : Ident.Map.t) (e : t) (h h' : heap) (v : value),
+        eval locals h e h' v ->
+        P locals h e h' v ->
+        P locals h (Mnumop1 (Malfunction.Neg, Float64, e)) h'
+          (Float (- as_float v))) ->
+       (forall (locals : Ident.Map.t) (h : heap) (x : t),
+        P locals h (Mnumop1 (Not, Float64, x)) h
+          (fail "invalid bitwise float operation")) ->
+       (forall (locals : Ident.Map.t) (h : heap) (x y : t)
+          (n : binary_bitwise_op),
+        P locals h (Mnumop2 (embed_binary_bitwise_op n, Float64, x, y)) h
+          (fail "invalid bitwise float operation")) ->
+       (forall (locals : Ident.Map.t) (h h1 h2 : heap) 
+          (op : binary_arith_op) (e1 e2 : t) (v1 v2 : value),
+        eval locals h e1 h1 v1 ->
+        P locals h e1 h1 v1 ->
+        eval locals h1 e2 h2 v2 ->
+        P locals h1 e2 h2 v2 ->
+        let v1' := as_float v1 in
+        let v2' := as_float v2 in
+        P locals h (Mnumop2 (embed_binary_arith_op op, Float64, e1, e2)) h2
+          (Float (binary_op_to_float op v1' v2'))) ->
+       (forall (locals : Ident.Map.t) (h h1 h2 : heap)
+          (op : binary_comparison) (e1 e2 : t) (v1 v2 : value),
+        eval locals h e1 h1 v1 ->
+        P locals h e1 h1 v1 ->
+        eval locals h1 e2 h2 v2 ->
+        P locals h1 e2 h2 v2 ->
+        let v1' := as_float v1 in
+        let v2' := as_float v2 in
+        let res := binary_comparison_to_bool op v1' v2' in
+        P locals h (Mnumop2 (embed_binary_comparison op, Float64, e1, e2)) h2
+          (value_Int (Int, if res then 1%Z else 0%Z))) ->
+       (forall (locals : Ident.Map.t) (h h' : heap) 
+          (e : t) (v : value) (src dst : inttype),
+        eval locals h e h' v ->
+        P locals h e h' v ->
+        P locals h (Mconvert (embed_inttype src, embed_inttype dst, e)) h'
+          (truncate dst (as_ty src v))) ->
+       (forall (locals : Ident.Map.t) (h h' : heap) 
+          (e : t) (v : value) (src : inttype),
+        eval locals h e h' v ->
+        P locals h e h' v ->
+        P locals h (Mconvert (embed_inttype src, Float64, e)) h'
+          (Float (of_uint63 (Int63.of_Z (as_ty src v))))) ->
+       (forall (locals : Ident.Map.t) (h h' : heap) (v : value) (e : t),
+        eval locals h e h' v ->
+        P locals h e h' v ->
+        P locals h (Mconvert (Float64, Float64, e)) h' (Float (as_float v))) ->
+       (forall (locals : Ident.Map.t) (h h1 h2 : heap)
+          (h3 h4 : heapGen value) (len : t) (len' : Z) 
+          (def : t) (def' : value) (ptr : pointer),
+        eval locals h len h1 (value_Int (Int, len')) ->
+        P locals h len h1 (value_Int (Int, len')) ->
+        eval locals h1 def h2 def' ->
+        P locals h1 def h2 def' ->
+        fresh h2 ptr h3 ->
+        update h3 ptr (init (Z.to_nat len') (fun _ : nat => def')) h4 ->
+        P locals h (Mvecnew (Array, len, def)) h4 (Vec (Array, ptr))) ->
+       (forall (locals : Ident.Map.t) (h h1 h2 : heap)
+          (h3 h4 : heapGen value) (len : t) (len' : Z) 
+          (def : t) (k : Z) (ptr : pointer),
+        eval locals h len h1 (value_Int (Int, len')) ->
+        P locals h len h1 (value_Int (Int, len')) ->
+        eval locals h1 def h2 (value_Int (Int, k)) ->
+        P locals h1 def h2 (value_Int (Int, k)) ->
+        fresh h2 ptr h3 ->
+        update h3 ptr
+          (init (Z.to_nat len') (fun _ : nat => value_Int (Int, k))) h4 ->
+        P locals h (Mvecnew (Bytevec, len, def)) h4
+          (if ((0 <=? k)%Z && (k <? 256)%Z)%bool
+           then Vec (Bytevec, ptr)
+           else fail "bad vector creation")) ->
+       (forall (locals : Ident.Map.t) (h h1 h2 : heap) 
+          (vec : t) (ty' : vector_type) (idx : t) 
+          (idx' : value) (ty : vector_type) (ptr : pointer)
+          (arr : list value),
+        eval locals h vec h1 (Vec (ty', ptr)) ->
+        P locals h vec h1 (Vec (ty', ptr)) ->
+        eval locals h1 idx h2 idx' ->
+        P locals h1 idx h2 idx' ->
+        deref h ptr arr ->
+        P locals h (Mvecget (ty, vec, idx)) h2
+          match idx' with
+          | value_Int (Int, i) =>
+              if vector_type_eqb ty ty'
+              then
+               if
+                ((0 <=? i)%Z && (i <? Z.of_nat (Datatypes.length arr))%Z)%bool
+               then nth (Z.to_nat i) arr (fail "")
+               else fail "index out of bounds: %d"
+              else fail "wrong vector type"
+          | _ => fail "wrong vector type"
+          end) ->
+       (forall (locals : Ident.Map.t) (h h1 h2 h3 : heap)
+          (h4 : heapGen value) (vec : t) (ty ty' : vector_type)
+          (ptr : pointer) (idx : t) (i : Z) (e : t) 
+          (v : value) (arr : list value),
+        eval locals h vec h1 (Vec (ty', ptr)) ->
+        P locals h vec h1 (Vec (ty', ptr)) ->
+        eval locals h1 idx h2 (value_Int (Int, i)) ->
+        P locals h1 idx h2 (value_Int (Int, i)) ->
+        eval locals h2 e h3 v ->
+        P locals h2 e h3 v ->
+        deref h ptr arr ->
+        update h3 ptr (set arr (Z.to_nat i) v) h4 ->
+        P locals h (Mvecset (ty, vec, idx, e)) h4
+          (if vector_type_eqb ty ty'
+           then
+            let i0 := Int63.of_Z i in
+            if
+             ((int_of_nat 0 ≤? i0)%uint63 &&
+              (i0 ≤? int_of_nat (Datatypes.length arr))%uint63)%bool
+            then
+             match ty with
+             | Array => value_Int (Int, 0%Z)
+             | Bytevec =>
+                 match v with
+                 | value_Int (Int, val) =>
+                     if ((0 <=? val)%Z && (val <? 256)%Z)%bool
+                     then value_Int (Int, 0%Z)
+                     else fail "not a byte"
+                 | _ => fail "not a byte"
+                 end
+             end
+            else fail "index out of bounds: %d"
+           else fail "wrong vector type")) ->
+       (forall (locals : Ident.Map.t) (h h' : heap) 
+          (vec : t) (ty' : vector_type) (ptr : pointer) 
+          (ty : vector_type) (arr : list value),
+        eval locals h vec h' (Vec (ty', ptr)) ->
+        P locals h vec h' (Vec (ty', ptr)) ->
+        deref h ptr arr ->
+        P locals h (Mveclen (ty, vec)) h'
+          (if vector_type_eqb ty ty'
+           then value_Int (Int, Z.of_nat (Datatypes.length arr))
+           else fail "wrong vector type")) ->
+forall (locals : Ident.Map.t) (h : heap) (t : t) 
          (h0 : heap) (v : value), eval locals h t h0 v -> P locals h t h0 v.
 Proof.
-  intros P H_lambda_sing H_lambda H_app_sing Happ_sing_rec H_app_fail H_app H_var H_let_body H_let_unnamed H_let_named 
-        H_let_rec H_switch H_block H_field H_field_fail H_lazy H_force_done H_force H_force_fail H_global.
-  fix f 6. intros locals h t h' v [| | | | | | | | | | | | ? ? ? ? ? Hforall | | | | | | | ].
-  1-12, 15-20:eauto.
-    - eapply H_block; eauto. induction Hforall; try econstructor; eauto. 
+  intros. 
+  revert locals h t h0 v H38.
+  fix f 6. intros locals h t h' v [| | | | | | | | | | | | ? ? ? ? ? Hforall | | | | | | | | | | | | | | | | | | | | | | | | | |].
+  1-12, 15-39:eauto.
+  - eapply H11; eauto. induction Hforall; try econstructor; eauto. 
     eapply IHHforall. cbn in *. lia.  
-  - eapply H_field. 1: eauto. 1: eauto. all: lia.
+  - eapply H12. 1: eauto. 1: eauto. all: lia.
 Qed.
 Set Elimination Schemes.
 
-(*
-
-Lemma int_of_to_nat i :
-  Int63_of_nat (int_to_nat i) = i.
-Proof.
-  unfold Int63_of_nat, int_to_nat.
-  rewrite Z2Nat.id.
-  1:eapply Int63.to_Z_bounded.
-  now rewrite Int63.of_to_Z.
-Qed.
-
-Lemma int_to_of_nat i :
-  (Z.of_nat i < Int63.wB)%Z ->
-  int_to_nat (Int63_of_nat i) = i.
-Proof.
-  unfold Int63_of_nat, int_to_nat.
-  intros ?.
-  rewrite Int63.of_Z_spec.
-  rewrite Z.mod_small. 1:lia.
-  now rewrite Nat2Z.id.
-Qed.
-
-Lemma Array_of_list'_get {A} s l (a : array A) i :
-  i < s + List.length l ->
-  (s + List.length l < Z.to_nat Int63.wB) ->
-  s + List.length l <= int_to_nat (PArray.length a) ->
-  PArray.get (Array_of_List' s l a) (Int63_of_nat i) =
-    if (i <? s)%nat then
-      a.[Int63_of_nat i]
-    else
-      nth (i - s) l (a.[Int63_of_nat i]).
-Proof.
-  intros Hl Hs Ha.
-  induction l as [ | ? ? IHl] in s, i, a, Hl, Hs, Ha |- *.
-  - destruct (Nat.ltb_spec i s).
-    + cbn. reflexivity.
-    + cbn. destruct (i - s); reflexivity.
-  - rewrite IHl. 
-    + cbn in Hl. lia.
-    + cbn [Datatypes.length] in Hs. lia.
-    + rewrite PArray.length_set. cbn [Datatypes.length] in Ha. lia.
-    + fold (Int63_of_nat s). destruct (Nat.ltb_spec i s) as [H | H].
-      * destruct (Nat.ltb_spec i (S s)) as [H0 | H0]; try lia.
-        rewrite get_set_other.
-        -- intros E. eapply (f_equal int_to_nat) in E.
-           rewrite !int_to_of_nat in E.
-           all:assert (H1 : s < Z.to_nat Int63.wB) by lia.
-           all:eapply inj_lt in H1.
-           all:rewrite Z2Nat.id in H1. all:lia. 
-        -- reflexivity.
-      * destruct (Nat.ltb_spec i (S s)); try lia.
-        -- assert (i = s) by lia. subst.
-           rewrite get_set_same.
-           ++ eapply Int63.ltb_spec.
-              1:eapply Z2Nat.inj_lt.
-              1:eapply Int63.to_Z_bounded.
-              1:eapply Int63.to_Z_bounded. 
-              fold (int_to_nat (Int63_of_nat s)).
-              rewrite int_to_of_nat. 1:lia.
-              unfold int_to_nat in Ha. lia.
-           ++ cbn. destruct s. 1:reflexivity.
-              rewrite Nat.sub_diag. reflexivity.
-        -- cbn. destruct (i - s) as [ | n] eqn:E.
-           ++ lia.
-           ++ assert (H1 : i - S s = n) by lia. rewrite H1.
-              eapply nth_indep.
-              cbn in Hl. lia.
-Qed.
-
-Lemma Array_of_list_get {A} (a : A) l i :
-  (i < Z.to_nat Int63.wB) ->
-  (List.length l < Z.to_nat Int63.wB) ->
-  List.length l <= int_to_nat max_length ->
-  i < List.length l ->
-  (Array_of_list a l).[Int63_of_nat i] = nth i l a.
-
-Proof.
-  unfold Array_of_list. intros Hs Hl1 Hl Hi.
-  rewrite Array_of_list'_get.
-  + assumption.
-  + lia. 
-  + rewrite PArray.length_make.
-    fold (Int63_of_nat (Datatypes.length l)).
-    destruct (Int63.lebP (Int63_of_nat (Datatypes.length l)) max_length) as [ | n ].
-    * rewrite int_to_of_nat.
-      1:eapply Z2Nat.inj_lt. all: lia. 
-    * destruct n.
-      epose proof (int_to_of_nat (Datatypes.length l) _) as H.
-      eapply Z2Nat.inj_le.
-      1:eapply Int63.to_Z_bounded.
-      1:eapply Int63.to_Z_bounded.
-      unfold int_to_nat in H. rewrite H.
-      unfold int_to_nat in Hl. exact Hl.
-      Unshelve. all:lia.
-  + destruct (Nat.ltb_spec i 0); try lia.
-    rewrite Nat.sub_0_r.
-    eapply nth_indep. lia.
-Qed.
-
-Lemma existsb_ext {A} (f g : A -> bool) l :
-  (forall x, f x = g x) ->
-  existsb f l = existsb g l.
-Proof.
-  intros H; induction l; cbn; congruence.
-Qed.
-
-Lemma Array_of_list_get_again {A : Set} i s (l : list A) a :
-  i >= s + List.length l ->
-  s + List.length l < Z.to_nat Int63.wB ->
-  i < Z.to_nat Int63.wB ->
-  (Array_of_List' s l a).[Int63_of_nat i]  = PArray.get a (Int63_of_nat i).
-Proof.
-  induction l as [ | ? l IHl ] in s, i, a |- *; intros Hi Hs Ha.
-  - cbn. reflexivity.
-  - cbn. rewrite IHl. 
-    + cbn in Hi. lia.
-    + cbn [List.length] in Hs. lia. 
-    + cbn [List.length] in Hs. lia.
-    + rewrite get_set_other. 2:reflexivity.
-      fold (Int63_of_nat s).
-      intros H. eapply (f_equal int_to_nat) in H.
-      rewrite !int_to_of_nat in H.
-      * eapply inj_lt in Hs.
-        rewrite Z2Nat.id in Hs. 1:cbn; lia.
-        rewrite <- Hs.
-        eapply inj_lt. cbn. lia.
-      * eapply inj_lt in Ha.
-        rewrite Z2Nat.id in Ha. 1:cbn; lia.
-        lia.
-      * subst. cbn in Hi. lia.
-Qed.
-
-End eval.
-
-
-Inductive vrel `{CompatiblePtr} (globals: @Ident.Map.t Interpreter.value) 
-    : value -> Interpreter.value -> Prop :=
-  | vBlock : forall tag vals vals', Forall2Array (vrel globals) vals vals' (fail "") ->
-      vrel globals (Block (tag, vals)) (Interpreter.Block (tag, vals'))
-  | vVec : forall ty ptr ptr', R_ptr ptr ptr' -> vrel globals (Vec (ty, ptr)) (Interpreter.Vec (ty, ptr'))
-  | vBString : forall ty ptr ptr', R_ptr ptr ptr' -> vrel globals (BString (ty, ptr)) (Interpreter.BString (ty, ptr'))
-  | vFunc : forall f x locals locals' e,  
-    (forall x, vrel globals (locals x) (locals' x)) ->
-    (forall h v, interpret h globals (Ident.Map.add x v locals') e = f h v) -> 
-    vrel globals (Func (locals,x,e)) (Interpreter.Func f)
-(*  | vFunc : forall (f : Interpreter.heap -> Interpreter.value -> Interpreter.heap * Interpreter.value)  x locals locals' e,  
-    (forall x, vrel eval (locals x) (locals' x)) ->
-    (forall h h' ih v v' res, vrel eval v v' -> eval (Ident.Map.add x v locals) h e h' res -> 
-      let (ih', res') := f ih v' in R_heap h' ih' /\ vrel eval res res') -> 
-    vrel eval (Func (x,locals,e)) (Interpreter.Func f)*)
-  | vRClos : forall f mfix n locals locals',  
-    (forall x, vrel globals (locals x) (locals' x)) ->
-    (*  (forall h v, interpret h globals (Ident.Map.add x v (add_all mfix E locals') locals') e = f h v) -> *)
-    vrel globals (RClos (locals,mfix,n)) (Interpreter.Func f)
-  | vInt : forall ty i , 
-      vrel globals (value_Int (ty, i)) (Interpreter.value_Int (ty, i))
-  | vFloat : forall f, 
-      vrel globals (Float f) (Interpreter.Float f)
-  | vThunk : forall ptr ptr', R_ptr ptr ptr' -> 
-      vrel globals (Thunk ptr) (Interpreter.Thunk ptr')
-  | vLazy : forall f e locals locals',  
-    (forall x, vrel globals (locals x) (locals' x)) ->
-    (forall h v, f h v = interpret h globals locals' e) -> 
-    vrel globals (Lazy (locals, e)) (Interpreter.Func f)
-  | vFail : forall s, 
-      vrel globals (fail s) (Interpreter.fail s)
-  | vNot_evaluated : vrel globals not_evaluated Interpreter.not_evaluated.
-
-Definition vrel_locals `{CompatiblePtr} (globals: @Ident.Map.t Interpreter.value) 
-  : Ident.Map.t -> Ident.Map.t -> Prop := fun locals ilocals => forall x, vrel globals (locals x) (ilocals x).
-
-Class CompatibleHeap `{CompatiblePtr} :=  
-  { R_heap : heap -> Interpreter.heap -> Prop;
-    fresh_compat : forall h ptr h' ih, 
-      R_heap h ih -> fresh h ptr h' -> 
-      let (iptr,ih') := Interpreter.fresh ih in R_ptr ptr iptr /\ R_heap h' ih';
-    update_compat : forall globals default h ih ptr ptr' h' v v', 
-      R_heap h ih -> update h ptr v h' -> 
-      R_ptr ptr ptr' -> Forall2Array (vrel globals) v v' default ->
-      let ih' := Interpreter.update ih ptr' v' in R_heap h' ih';
-    deref_compat : forall globals default h ih ptr ptr' vals, 
-      R_heap h ih -> deref h ptr vals -> 
-      R_ptr ptr ptr' -> 
-      let vals' := Interpreter.deref ih ptr' in 
-      Forall2Array (vrel globals) vals vals' default 
-   }.
-
-
-Lemma Forall2_acc_map {S S' A B B'} (R : S -> S' -> Prop) (RB : B -> B' -> Prop)
-        (f : S' -> A -> S' * B') (P : S -> A -> S -> B -> Prop) x x' y l1 l2 :
-  Forall2_acc P x l1 y l2 ->
-  (forall x x' a b y, R x x' -> P x a y b -> let (y' , b') := f x' a in R y y' /\ RB b b') ->
-  R x x' -> 
-  let (y' , l') := map_acc f x' l1 in R y y' /\ Forall2 RB l2 l'.
-Proof.
-  intros H H'. revert x'. induction H; cbn; intros x' Hx; f_equal; eauto.
-  specialize (H' _ _ _ _ _ Hx H). destruct (f _ _ ) as (s',b').
-  destruct H'. specialize (IHForall2_acc _ H1). destruct (map_acc _ _ _).
-  destruct IHForall2_acc. split; eauto.  
-Qed.
-
-Lemma cond_correct  `{CompatiblePtr} 
-  globals' scr scr' x : vrel globals' scr scr' -> 
-  cond scr x = Interpreter.cond scr' x.
-Proof.
-  now destruct x as [ | | [] ]; destruct 1. 
-Qed.
-
-Lemma find_match_correct `{CompatiblePtr}  scr scr' cases e h iglobals ilocals :
-  vrel iglobals scr scr' ->
-  find_match scr cases = Some e ->
-  Interpreter.find_match Interpreter.interpret h iglobals ilocals scr' cases = interpret h iglobals ilocals e.
-Proof.
-  induction cases as [ | a cases IHcases ]; cbn [find_match]; intros rel Eq.
-  - inversion Eq.
-  - destruct a.
-    cbn [Interpreter.find_match].
-    destruct existsb eqn:E.
-    * inversion Eq. subst.
-      erewrite existsb_ext.
-      2:{ intros. symmetry. eapply cond_correct. eauto.  }
-      now rewrite E.
-    * erewrite existsb_ext.
-      2:{ intros. symmetry. eapply cond_correct. eauto. }
-      rewrite E. eauto.
-Qed.
-
-Axiom todo : forall {A : Type}, A.
-
-Ltac fail_case IHeval Hloc Hheap Heq := 
-  let Hv := fresh "iv1" in cbn; specialize (IHeval _ _ Hloc Hheap); destruct interpret as [? ?];
-  destruct IHeval as [? Hv]; destruct Hv; inversion Heq; split;eauto; econstructor.
-
-Lemma vrel_add `{CompatiblePtr} iglobals x v iv locals ilocals : vrel iglobals v iv -> vrel_locals iglobals locals ilocals -> 
-  vrel_locals iglobals (Ident.Map.add x v locals) (Ident.Map.add x iv ilocals).
-Proof.
-  intros Hv Hlocals nm. unfold Ident.Map.add. now destruct Ident.eqb.
-Qed.
-
-Lemma Array_of_list_S A default n a (l:list A) : 
-  n < Datatypes.length l ->
-  S (Datatypes.length l) <= int_to_nat max_length ->
-  (Array_of_list default (a :: l)).[Int63_of_nat (S n)] = 
-  (Array_of_list default l).[Int63_of_nat n].
-Proof.
-  intros. 
-  repeat rewrite Array_of_list_get; cbn in *; try lia; eauto.
-Qed. 
-
-Lemma Array_of_list'_length A k (l:list A) a :
-  PArray.length (Array_of_List' k l a) =
-  PArray.length a.
-Proof. 
-  revert k a. induction l; [reflexivity|].
-  intros; cbn. rewrite IHl. now rewrite PArray.length_set.
-Qed.    
-
-Lemma Array_of_list_length A default (l:list A) :
-  Datatypes.length l < int_to_nat max_length -> 
-  int_to_nat (PArray.length (Array_of_list default l)) =
-  List.length l.
-Proof.
-  unfold Array_of_list. rewrite Array_of_list'_length.
-  rewrite PArray.length_make. intro H. 
-  assert (Hl: (Int63_of_nat (Datatypes.length l) ≤? max_length)%uint63 = true).
-  { apply leb_spec. rewrite Int63.of_Z_spec. rewrite Z.mod_small; [cbn in *; lia |].
-    cbn in *; lia. }
-  rewrite Hl. apply int_to_of_nat. cbn in *; lia. 
-Qed.    
-  
-Lemma Forall2_acc_length {X A B R x l y l'} : @Forall2_acc X A B R x l y l' -> List.length l = List.length l'.
-Proof. 
-  induction 1; cbn; eauto.
-Qed.   
-
-Lemma Forall2_length {A B P l l'} : @Forall2 A B P l l' -> List.length l = List.length l'.
-Proof. 
-  induction 1; cbn; eauto.
-Qed.
-
-Lemma isNotEvaluated_vrel `{CompatiblePtr} iglobals v v' b : 
-  vrel iglobals v v' -> isNotEvaluated v = b <-> is_not_evaluated v' = b.
-Proof.
-  now destruct 1.
-Qed.    
-
-Axiom funext : forall A B, forall f g : A -> B, (forall x, f x = g x) -> f = g.
-
-Lemma interpret_ilocals_proper `{CompatiblePtr} ih iglobals ilocals ilocals' e :
-  (forall x, ilocals x = ilocals' x) ->
-  interpret ih iglobals ilocals e = interpret ih iglobals ilocals' e.
-Proof.
-  intros Hlocal; apply funext in Hlocal. now subst.
-Qed.  
-  
-Lemma eval_correct `{CompatibleHeap} 
-  globals locals ilocals iglobals e h h' ih v :
-  (forall nm val, In (nm, val) globals -> vrel iglobals val (iglobals nm)) ->
-  vrel_locals iglobals locals ilocals ->
-  R_heap h ih ->
-  eval _ globals locals h e h' v -> 
-  let (ih',iv) := interpret ih iglobals ilocals e in R_heap h' ih' /\ vrel iglobals v iv.  
-Proof.
-  rename H into _Heap; rename H0 into _iHeap; rename H1 into _CPtr; rename H2 into _CHeap. 
-  intros Hglob Hloc Hheap.
-  induction 1 as [ (* lambda_sing *) locals h x e
-                 | (* lambda *) locals h x ids e H
-                 | (* app_sing *) locals h1 h2 h3 h4 x locals' e e2 v2 e1 v H IHeval1 H0 IHeval2 H1 IHeval3
-                 | (* app_fail *) locals h h' e2 e v Heval IHeval Heq
-                 | (* app *) locals h h' e2 e1 v vals tag IHeval 
-                 | (* var *) 
-                 | (* let_body *) | (* let_unnamed *) | (* let_named *) | (* let_rec *)
-                 | (* switch *) 
-                 | (* block *)  
-                 | (* field *) locals h h' idx b vals tag H IHeval | | | | | | ]
-                 in ih, Hheap, ilocals, Hloc |- *. 
-  (* eval_lambda_sing *) 
-  - split; eauto. econstructor; eauto.
-  (* eval_lambda *)
-  - split; eauto. 
-    destruct ids as [ | t ids ]; cbn in H. 1:inversion H. clear H.
-    econstructor; eauto.  
-  (* eval_app_sing *)
-  - cbn; specialize (IHeval1 _ _ Hloc Hheap). destruct interpret as [ih1 iv1]; destruct IHeval1 as [Hheap1  Hiv1].
-    specialize (IHeval2 _ _ Hloc Hheap1). destruct interpret as [ih2 iv2]; destruct IHeval2 as [Hheap2  Hiv2].
-    inversion Hiv1 ; subst. rewrite <- H7. clear H7 f Hiv1.
-    specialize (IHeval3 (Ident.Map.add x iv2 locals'0) ih2). 
-    destruct interpret as [ih3 iv3]; cbn in *.
-    apply IHeval3; eauto. now apply vrel_add. 
-  (* eval_app_fail *)
-  - fail_case IHeval Hloc Hheap Heq.
-  (* eval_app *)
-  - now apply IHeval.
-  (* eval_var *)
-  - cbn; eauto.
-  (* eval_let_body *)
-  - now eapply IHeval.
-  (* eval_let_unnamed *)
-  - cbn; specialize (IHeval1 _ _ Hloc Hheap). destruct interpret as [ih1 iv1]; destruct IHeval1 as [Hheap1  Hiv1].
-    now eapply IHeval2. 
-  (* eval_let_named *)
-  - cbn; specialize (IHeval1 _ _ Hloc Hheap). destruct interpret as [ih1 iv1]; destruct IHeval1 as [Hheap1  Hiv1].
-    eapply IHeval2; eauto. now apply vrel_add. 
-  (* eval_let_rec *)
-  - cbn; eapply IHeval; eauto. intros x. clear IHeval.
-    clear - H Hloc. revert H.
-    unfold add_recs.
-    rewrite newlocals_eqn.
-    generalize recs at 1 3.
-    intros allrecs H.
-    induction recs as [ | (f, e) recs IH] in allrecs, ilocals, locals, H, newlocals, Hloc |- *.
-    + cbn in H |- *. inversion H as [E]; subst. eapply Hloc.
-    + cbn in H |- *. destruct e; try now inversion H.
-      destruct p as (bindings, e).
-      destruct bindings as [ | y ]; try now inversion H.
-      destruct add_recs' as [ newlocals' | ] eqn:E; inversion H. subst. clear H. 
-      unfold Ident.Map.add, Ident.eqb.
-      destruct (String.eqb_spec x f).
-      2: eapply IH; eauto.
-      subst. cbn.  clear IH. econstructor; [eauto|].
-      intros ih iv. cbn. 
-      enough (
-        interpret ih iglobals
-        (Ident.Map.add y iv
-           (fun x : Ident.t => newlocals (fun h => interpret h iglobals) allrecs ilocals x))
-        (Mklambda bindings e) =
-      interpret ih iglobals (Ident.Map.add y iv ilocals)
-        (Mlet ([Recursive allrecs], Mklambda bindings e))) by (destruct bindings; eauto).
-      generalize (Mklambda bindings e). clear e. intros e. cbn.
-      clear E. apply interpret_ilocals_proper. intros.
-      assert (~(In y (map fst allrecs))) by apply todo.
-      unfold Ident.Map.add. 
-      case_eq (Ident.eqb x y); cbn.
-      * intro eqxy. rewrite eqb_eq in eqxy. subst. 
-        enough (forall allrecs y l, ~ In y (map fst allrecs) ->
-          newlocals (fun h : Interpreter.heap => interpret h iglobals) allrecs l y = l y).
-         ** rewrite H0; eauto. unfold Ident.eqb. now rewrite String.eqb_refl.
-         ** clear. intros. rewrite newlocals_eqn.
-            generalize allrecs at 1. revert y H. 
-            induction allrecs; cbn; intros; [reflexivity|].
-            destruct a. unfold Ident.Map.add. 
-            rewrite not_in_cons in H; destruct H. cbn in H. 
-            assert (Ident.eqb y t = false) by now rewrite eqb_neq.
-            rewrite H1. apply IHallrecs; eauto. 
-      * intro neqxy. pose proof (H' := H). revert H' H. repeat rewrite newlocals_eqn.
-        generalize allrecs at 2 3 5.
-        induction allrecs.
-        ** cbn. now rewrite neqxy.
-        ** cbn. intro. 
-           rewrite not_in_cons; intros.
-           destruct a. unfold Ident.Map.add.
-           case_eq (Ident.eqb x t).
-          *** intro. destruct t0; try reflexivity.
-            f_equal. apply funext. intro. apply funext.
-            intro. assert (forall t0, interpret x0 iglobals
-            (fun x2 : Ident.t =>
-                newlocals (fun h : Interpreter.heap => interpret h iglobals) allrecs0 ilocals x2) t0 =
-            interpret x0 iglobals
-            (fun x2 : Ident.t =>
-                newlocals (fun h : Interpreter.heap => interpret h iglobals) allrecs0
-                  (fun y0 : string => if Ident.eqb y0 y then iv else ilocals y0) x2) t0) by apply todo.
-            now rewrite H1.
-        *** destruct H. intro; apply IHallrecs; eauto.  
-  (* eval_switch *)
-  - cbn.
-    specialize (IHeval1 _ _ Hloc Hheap). destruct interpret as [ih1 iv1]; destruct IHeval1 as [Hheap1  Hiv1].
-    erewrite find_match_correct; eauto. now apply IHeval2.
-  (* eval_block *)
-  - cbn. clear H. revert ih Hheap. induction H1. 
-    + intros ih Hheap. split ; eauto. econstructor.
-      split; [ reflexivity|]. cbn. lia.
-    + intros ih Hheap. simpl. 
-      specialize (H _ _ Hloc Hheap). destruct interpret as [ih1 iv1]; destruct H as [Hheap1  Hiv1]. 
-      assert (Hlength: Datatypes.length l' < int_to_nat max_length) by (cbn in *; lia). 
-      specialize (IHForall2_acc Hlength ih1 Hheap1).     
-      unshelve epose proof (Forall2_acc_map R_heap (vrel iglobals)
-        (fun (h : Interpreter.heap) (e : t) => interpret h iglobals ilocals e) _ _ _ _ _ _ H1 _ Hheap1).
-      { clear -Hloc. intros. cbn in *. specialize (H0 ilocals x'). destruct interpret. apply H0; eauto. }
-      set (p := map_acc _ ih1 l) in *. destruct p. destruct H as [Heahp2 Hl0]. split; eauto. 
-      destruct IHForall2_acc as [? IHForall2_acc]. 
-      assert (Hl: (Int63_of_nat (Datatypes.length l) ≤? max_length)%uint63 = true).
-      { apply leb_spec. rewrite Int63.of_Z_spec.
-        rewrite (Forall2_acc_length H1). rewrite Z.mod_small; [cbn in *; lia |]. cbn in *; lia. } 
-      assert (Hl': (Int63_of_nat (S (Datatypes.length l)) ≤? max_length)%uint63 = true).
-      { apply leb_spec. rewrite Int63.of_Z_spec. rewrite (Forall2_acc_length H1). rewrite Z.mod_small; [cbn in *; lia |].
-        cbn in *; lia. } 
-      rewrite Hl in IHForall2_acc. rewrite Hl'. inversion IHForall2_acc; subst. clear IHForall2_acc.  
-      econstructor. destruct H3. split.
-      * simpl. rewrite Array_of_list_length.
-        { cbn. rewrite <- (Forall2_length Hl0). clear - H0; cbn in *; lia. }
-        now rewrite (Forall2_length Hl0).
-      * intros idx Hidx. rewrite <- (int_of_to_nat idx) at 2.
-        pose proof (Hbounded := to_Z_bounded idx).
-        destruct (int_to_nat idx).
-        ** simpl. pose Int63.wB_pos. rewrite Array_of_list_get; try (cbn; lia).
-          ++ cbn in H0. rewrite (Forall2_length Hl0) in H0. clear - H0; cbn in *; lia. 
-          ++ cbn in H0. rewrite (Forall2_length Hl0) in H0. clear - H0; cbn in *; lia. 
-          ++ eauto.
-        ** simpl. rewrite Array_of_list_S. 
-           ++ cbn; cbn in Hidx. rewrite <- (Forall2_length Hl0). lia.
-           ++ cbn; cbn in H0. rewrite <- (Forall2_length Hl0). lia.
-           ++ specialize (H3 (Int63_of_nat n)). 
-              rewrite int_to_of_nat in H3.
-              { cbn; cbn in Hidx; cbn in H0. lia. }
-              eapply H3. cbn in Hidx; lia.  
-  (* eval_field *)    
-  - cbn. specialize (IHeval _ _ Hloc Hheap). destruct interpret as [ih1 iv1]; destruct IHeval as [Hheap1  Hiv1].
-    split; eauto. inversion Hiv1; subst. clear Hiv1. destruct H6 as [? H5]. 
-    now eapply (H5 idx).  
-  (* eval_field_fail *)    
-  - fail_case IHeval Hloc Hheap H0.
-  (* eval_lazy *)  
-  - cbn. pose proof (fresh_compat _ _ _ _ Hheap H).
-    set (Interpreter.fresh ih) in *. destruct p.
-    destruct H1; split; [| now econstructor].
-    eapply update_compat with (default := fail ""); eauto. split; [reflexivity|].
-    intros idx Hidx. rewrite <- (int_of_to_nat idx). destruct int_to_nat. 
-    * cbn. econstructor; eauto.
-    * cbn in Hidx. lia.
-  (* eval_force_done *)  
-  - cbn. specialize (IHeval _ _ Hloc Hheap). destruct interpret as [ih1 iv1]; destruct IHeval as [Hheap1  Hiv1]. 
-    inversion Hiv1; subst; clear Hiv1.
-    pose proof (deref_compat iglobals (fail "") _ _ _ _ _ Hheap1 H0 H5).
-    destruct H1 as [? Hderef]. pose proof (Hderef (int_of_nat 0) H2).
-    cbn in H4. rewrite isNotEvaluated_vrel in H3; eauto. 
-    now destruct is_not_evaluated; inversion H3.
-  (* eval_force *)  
-  - cbn; specialize (IHeval1 _ _ Hloc Hheap). destruct interpret as [ih1 iv1]; destruct IHeval1 as [Hheap1  Hiv1].
-    inversion Hiv1; subst; clear Hiv1.
-    pose proof (deref_compat iglobals (fail "") _ _ _ _ _ Hheap1 H0 H7).
-    destruct H6 as [? Hderef]. pose proof (Hderef (int_of_nat 0)).
-    cbn in H8. rewrite isNotEvaluated_vrel in H1; [eapply H8; lia|]. 
-    destruct is_not_evaluated; inversion H1. clear H1. rewrite H3 in Hderef. 
-    pose proof (Hderef (int_of_nat 1) (ltac:(eauto))). cbn in H1.
-    rewrite H2 in H1. set _.[1] in *.  inversion H1; subst; clear H1.
-    rewrite H13.
-    specialize (IHeval2 _ _ H12 Hheap1). destruct interpret as [ih2 iv2]; destruct IHeval2 as [Hheap2  Hiv2].
-    split; eauto. 
-    eapply update_compat with (default := fail ""); eauto. split; cbn.   
-    * rewrite PArray.length_set. lia.
-    * intro i. pose proof (int_of_to_nat i). destruct (int_to_nat i); [| destruct  n].
-      + subst. intros _. rewrite get_set_same; eauto.
-        rewrite <- (int_of_to_nat (PArray.length _)). rewrite <- H6. 
-        rewrite H3. cbn; lia.
-      + subst; intros _. rewrite get_set_other; [now apply eqb_false_spec|]. cbn.
-        fold y. rewrite <- H11. econstructor; eauto.
-      + lia. 
-  (* eval_force_fail *)  
-  - fail_case IHeval Hloc Hheap H0.
-  - cbn. split; eauto. 
-  Qed.
-Set Guard Checking.
-
-
-(*  Lemma vtrans_inj v v' : vtrans v = vtrans v' -> v = v'.
-  Admitted. 
-  Lemma apD {A B} {f g : forall a:A, B a} : f = g -> forall x, f x = g x. 
-  now destruct 1.
-  Defined.  *)
-
-  Lemma interp_correct iglobals globals locals e v ilocals :
-    (forall x, vrel iglobals (ilocals x) (locals x)) ->
-    vrel (interpret ilocals e) v -> eval globals locals e v.
-  induction e; intro Hlocal; cbn in *. 
-  - intros Hvar. unfold Ident.Map.find in Hvar. rewrite Hlocal in Hvar.
-    apply vtrans_inj in Hvar. subst. econstructor. 
-  - intros Hlambda. destruct p as [xs e]. induction xs; cbn in *.
-    * admit.
-    * destruct xs.
-      + destruct v; cbn in Hlambda; try destruct p; try now inversion Hlambda.
-        destruct p. inversion Hlambda. clear Hlambda.
-        pose proof (Hlambda := apD H0 a). 
-        
-         H0. pose (ap )
-        f_equal
-        
-        eapply eval_lambda_sing. 
-           
-
-  destruct v. inversion Hvar.  eapply eval_var. 
-
-*)
 End eval.
