theories/Ceres/CeresSerialize.v
@@ -1,0 +1,95 @@
+(** * Serialization to S-expressions *)
+
+(* begin hide *)
+From Coq Require Import
+  List
+  ZArith
+  Ascii
+  String.
+
+From Ceres Require Import
+  CeresS
+  CeresString.
+
+From Malfunction Require Import 
+  CeresFormat.
+(* end hide *)
+
+From MetaCoq Require Import bytestring.
+
+(** Serialization to S-expressions. *)
+Class Serialize (A : Type) :=
+  to_sexp : A -> sexp.
+
+(** Serialize a value to a string. *)
+Definition to_string {A} `{Serialize A} : A -> string :=
+  fun a => string_of_sexp (to_sexp a).
+
+(** ** Serialize integers *)
+
+(** Integer representations. *)
+Class Integral (A : Type) :=
+  to_Z : A -> Z.
+
+(** Integers are serializable. *)
+Global
+Instance Serialize_Integral {A : Type} `(Integral A) : Serialize A :=
+  fun z => Atom (to_Z z).
+
+Global
+Instance Integral_nat : Integral nat := Z.of_nat.
+Global
+Instance Integral_N : Integral N := Z.of_N.
+Global
+Instance Integral_Z : Integral Z := id.
+
+(** ** Serialize common types *)
+
+Global
+Instance Serialize_bool : Serialize bool
+  := fun b => Atom (string_of_bool b).
+
+Global
+Instance Serialize_option {A} `(Serialize A) : Serialize (option A)
+  := fun oa =>
+    match oa with
+    | None => Atom "None"%string
+    | Some a => [ Atom "Some"%string ; to_sexp a ]%sexp
+    end.
+
+Global
+Instance Serialize_sum {A B} `(Serialize A) `(Serialize B)
+  : Serialize (A + B)
+  := fun ab =>
+    match ab with
+    | inl a => [ Atom "inl"%string ; to_sexp a ]%sexp
+    | inr b => [ Atom "inr"%string ; to_sexp b ]%sexp
+    end.
+
+Global
+Instance Serialize_product {A B} `(Serialize A) `(Serialize B)
+  : Serialize (A * B)
+  := fun ab => [ to_sexp (fst ab) ; to_sexp (snd ab) ]%sexp.
+
+Global
+Instance Serialize_Empty_set : Serialize Empty_set
+  := fun v => match v with end.
+
+Global
+Instance Serialize_unit : Serialize unit
+  := fun _ => Atom "tt"%string.
+
+Global
+Instance Serialize_ascii : Serialize ascii
+  := fun a => Atom (Str (String a "")).
+
+Global
+Instance Serialize_string : Serialize String.string
+  := fun s => Atom (Str s).
+
+Global
+Instance Serialize_list {A} `{Serialize A} : Serialize (list A)
+  := fun xs => List (List.map to_sexp xs).
+
+Global
+Instance Serialize_sexp : Serialize sexp := id.
