theories/Firstorder.v
@@ -1,0 +1,91 @@
+Require Import ssreflect.
+From Malfunction Require Import Malfunction SemanticsSpec.
+From MetaCoq.PCUIC Require Import PCUICAst PCUICFirstorder.
+
+Require Import ZArith Array.PArray List String Floats Lia Bool.
+Import ListNotations.
+
+
+Inductive camlType : Set :=
+    Arrow : camlType -> camlType -> camlType
+  | Rel : nat -> camlType 
+  | Const : kername -> 
+            (* number of ADT in the mutual definition *) nat -> 
+            (* list of parameters *) list camlType -> 
+            camlType.
+
+Notation "A → B" := (Arrow A B) (at level 50). 
+
+Definition ADT : Set := 
+  (* number of parameters *)
+  nat * list (
+  nat (* constructors w/o arguments *) *
+  list (list camlType) (* constrcutors w/ arguments *)).
+
+Section firstorder.
+
+  Context {Σb : list (kername * bool)}.
+
+  Definition CoqType_to_camlType_oneind_type n k decl_type :
+    is_true (@firstorder_type Σb k n decl_type) -> camlType.
+  Proof.
+    unfold firstorder_type. intro H.
+    destruct (fst _); inversion H.
+    (* case of tRel with a valid index *)
+
+    - exact (Rel n0).
+    (* case of tInd where Σb is saying that inductive_mind is first order *)
+    - destruct ind. exact (Const inductive_mind inductive_ind []).
+  Defined.  
+
+  Definition CoqType_to_camlType_oneind mind ind : 
+    ind_params mind = [] -> 
+    is_true (@firstorder_oneind Σb mind ind) -> nat * list (list camlType).
+  Proof.
+    destruct ind. intros Hparam H. apply MCProd.andb_and in H.
+    destruct H as [H _]. cbn in *. clear -H Hparam.
+    induction ind_ctors0.
+    (* no more constructor *)
+    - exact (O , []).
+    (* a :: ind_ctors0 constructors *)
+    - apply MCProd.andb_and in H. destruct H. destruct (IHind_ctors0 H0) as [n l].
+      (* [n l] codes for ind_ctors *)
+      destruct a. revert H. cbn. rewrite Hparam. generalize (rev (cstr_args0 ++ [])).
+      clear - n l.
+      intros cstr; generalize 0. destruct cstr; intros.
+      (* cstr is a constrcutor with no argument, we increment the number n *)
+      + exact (S n,l).
+      (* c :: cstr , we extend the list of list *)
+      + refine (n,_::l). clear n l.
+        revert n0 H. generalize (c::cstr). clear. 
+        intros cstr; induction cstr; cbn; intros. 
+        (* we convert the type of the first type of the constructor *)
+        * exact [].
+        * apply MCProd.andb_and in H. destruct H. destruct a.
+        (* we convert the type of the first type of the constructor *)
+          apply CoqType_to_camlType_oneind_type in H.
+          refine (H :: _). clear H.
+        (* we recursively convert *)
+          exact (IHcstr _ H0).
+    Defined.
+
+  (* The following function morally do (map CoqType_to_camlType_oneind) while passing 
+  th proof that everything is first order *)
+
+  Definition CoqType_to_camlType mind : 
+    ind_params mind = [] -> 
+    is_true (@firstorder_mutind Σb mind) -> ADT.
+  Proof.
+    (* no parameters *)
+    intros Hparam H. refine (0,_).
+    destruct mind. unfold firstorder_mutind; cbn. 
+    apply MCProd.andb_and in H. destruct H as [_ H].
+    revert H. generalize ind_bodies0 at 1. induction ind_bodies0; cbn in *; intros.
+    - exact [].
+    - apply MCProd.andb_and in H. destruct H. cbn in *. 
+      specialize (IHind_bodies0 Hparam _ H0). clear H0. refine (_ :: IHind_bodies0). 
+      apply (CoqType_to_camlType_oneind) in H; eauto.
+  Defined.
+
+End firstorder.
+
